Rename ETyping into EGlobalEnv, add EEnvMap module and restore EEtaExpanded, moving the one with fixpoints to EEtaExpandedFix

erasure/theories/EEtaExpanded.v
@@ -1,4 +1,7 @@
 (* Distributed under the terms of the MIT license. *)
+
+(* Eta expanded constructors only, see EEtaExpandedFix for the more involved definition where fixpoints are also eta-expanded. *)
+
 From Coq Require Import Utf8 Program.
 From MetaCoq.Template Require Import config utils Kernames EnvMap.
 From MetaCoq.PCUIC Require Import PCUICAst PCUICAstUtils
@@ -7,204 +10,11 @@ From MetaCoq.PCUIC Require Import PCUICAst PCUICAstUtils
      PCUICConfluence PCUICConversion 
      PCUICCumulativity PCUICSR PCUICSafeLemmata
      PCUICValidity PCUICPrincipality PCUICElimination PCUICSN.
-     
-
-From MetaCoq.Template Require Import config utils BasicAst Universes.
-From MetaCoq.Erasure Require Import EAst ETyping EAstUtils.
-From MetaCoq.Erasure Require Import EWcbvEval EWcbvEvalInd.
-
-Lemma eval_trans' {wfl : WcbvFlags} {Σ e e' e''} :
-  eval Σ e e' -> eval Σ e' e'' -> e' = e''.
-Proof.
-  intros ev ev'.
-  eapply eval_to_value in ev.
-  eapply value_final in ev.
-  eapply (eval_deterministic ev ev').
-Qed.
-
-Lemma eval_trans {wfl : WcbvFlags} {Σ e e' e''} :
-  eval Σ e e' -> eval Σ e' e'' -> eval Σ e e''.
-Proof.
-  intros ev ev'.
-  enough (e' = e'') by now subst.
-  eapply eval_trans'; eauto.
-Qed.
-
-Arguments eval : clear implicits.
-
-Lemma eval_app_cong_tApp {wfl : WcbvFlags} Σ t v args res :
-  eval target_wcbv_flags Σ t v ->  
-  eval target_wcbv_flags Σ (tApp v args) res ->
-  eval target_wcbv_flags Σ (tApp t args) res.
-Proof.
-  intros. depind H0.
-  - econstructor; eauto. eapply eval_trans; eauto.
-  - econstructor; eauto. eapply eval_trans; eauto.
-  - eapply eval_fix'; eauto. eapply eval_trans; eauto.
-  - eapply eval_app_cong; eauto. eapply eval_trans; eauto.
-  - cbn in i. easy.
-Qed.
-
-Definition isRel t :=
-    match t with tRel _ => true | _ => false end.
-
-Section expanded.
-
-Variable Σ : global_declarations.
-
-Local Unset Elimination Schemes.
- 
-Inductive expanded (Γ : list nat): term -> Prop :=
-| expanded_tRel_app (n : nat) args m : nth_error Γ n = Some m -> forall Hle : m <= #|args|, Forall (expanded Γ) args -> expanded Γ (mkApps (tRel n) args)
-| expanded_tVar (id : ident) : expanded Γ (tVar id)
-| expanded_tEvar (ev : nat) (args : list term) : Forall (expanded Γ) args -> expanded Γ (tEvar ev args)
-| expanded_tLambda (na : name) (body : term) : (* expanded Γ ty -> *) expanded (0 :: Γ) body -> expanded Γ (tLambda na body)
-| expanded_tLetIn (na : name) (def : term) (body : term) : expanded Γ def (* -> expanded Γ def_ty *) -> expanded (0 :: Γ) body -> expanded Γ (tLetIn na def body)
-| expanded_mkApps (f : term) (args : list term) : negb (isConstruct f || isFix f || isRel f) -> expanded Γ f -> Forall (expanded Γ) args -> expanded Γ (mkApps f args)
-| expanded_tConst (c : kername) : expanded Γ (tConst c)
-| expanded_tCase (ind : inductive) (pars : nat) (discr : term) (branches : list (list name × term)) :  
-    expanded Γ discr -> 
-    Forall (fun br => expanded (repeat 0 #|br.1| ++ Γ) br.2) branches -> 
-    expanded Γ (tCase (ind, pars) discr branches)
-| expanded_tProj (proj : projection) (t : term) : expanded Γ t -> expanded Γ (tProj proj t)
-| expanded_tFix (mfix : mfixpoint term) (idx : nat) args d : 
-  Forall (fun d => 
-           let ctx := rev_map (fun  d => 1 + d.(rarg)) mfix in
-          expanded (ctx ++ Γ) d.(dbody)) mfix ->
-  Forall (expanded Γ) args ->
-  args <> [] ->
-  nth_error mfix idx = Some d ->
-  #|args| > d.(rarg) ->
-  expanded Γ (mkApps (tFix mfix idx) args)
-| expanded_tCoFix (mfix : mfixpoint term) (idx : nat) : 
-  Forall (fun d => expanded (repeat 0 #|mfix| ++ Γ) d.(dbody)) mfix ->
-  expanded Γ (tCoFix mfix idx)
-| expanded_tConstruct_app ind idx mind idecl cname c args :
-    declared_constructor Σ (ind, idx) mind idecl (cname, c) ->
-    #|args| >= ind_npars mind + c -> 
-    Forall (expanded Γ) args ->
-    expanded Γ (mkApps (tConstruct ind idx) args)
-| expanded_tBox : expanded Γ tBox.
-
-End expanded.
-
-Lemma expanded_ind :
-  ∀ (Σ : global_declarations) (P : list nat → term → Prop),
-     (∀ (Γ : list nat) (n : nat) (args : list term) (m : nat),
-         nth_error Γ n = Some m ->
-          (m ≤ #|args|) ->
-	        Forall (expanded Σ Γ) args
-        → Forall (P Γ) args 
-        → P Γ (mkApps (tRel n) args)) →
-    (forall id : ident, forall Γ, P Γ (tVar id)) →
-    (forall (ev : nat) (args : list term) Γ, Forall (expanded Σ Γ) args → Forall (P Γ) args → P Γ (tEvar ev args)) 
-    → (∀ (Γ : list nat) (na : name) (body : term),
-          expanded Σ (0 :: Γ) body → P (0 :: Γ) body → P Γ (tLambda na body))
-    → (∀ (Γ : list nat) (na : name) (def body : term),
-          expanded Σ Γ def
-        → P Γ def
-        → expanded Σ (0 :: Γ) body
-        → P (0 :: Γ) body → P Γ (tLetIn na def body))
-    → (∀ (Γ : list nat) (f3 : term) (args : list term),
-          negb (isConstruct f3 || isFix f3 || isRel f3)
-        → expanded Σ Γ f3
-        → P Γ f3 → Forall (expanded Σ Γ) args → Forall (P Γ) args → P Γ (mkApps f3 args))
-    → (∀ (Γ : list nat) (c : kername), P Γ (tConst c))
-    → (∀ (Γ : list nat) (ind : inductive) 
-         (pars : nat) (discr : term) (branches : 
-                                     list 
-                                       (list name × term)),
-          expanded Σ Γ discr
-        → P Γ discr
-        → Forall
-            (λ br : list name × term,
-                expanded Σ (repeat 0 #|br.1| ++ Γ) br.2) branches
-        → Forall
-            (λ br : list name × term,
-                P (repeat 0 #|br.1| ++ Γ) br.2) branches
-        → P Γ (tCase (ind, pars) discr branches))
-    → (∀ (Γ : list nat) (proj : projection) (t : term),
-          expanded Σ Γ t → P Γ t → P Γ (tProj proj t))
-    → (∀ (Γ : list nat) (mfix : mfixpoint term) 
-         (idx : nat) (args : list term) 
-         (d : def term),
-          Forall
-            (λ d0 : def term,
-                let ctx := rev_map (fun  d => 1 + d.(rarg)) mfix in
-                expanded Σ (ctx ++ Γ) (dbody d0)) mfix
-          → Forall
-            (λ d0 : def term,
-               let ctx := rev_map (fun  d => 1 + d.(rarg)) mfix in
-                P (ctx ++ Γ) (dbody d0)) mfix
-          → Forall (expanded Σ Γ) args
-          → Forall (P Γ) args
-          → args ≠ []
-          → nth_error mfix idx = Some d
-          → #|args| > rarg d
-                    → P Γ (mkApps (tFix mfix idx) args))
-    → (∀ (Γ : list nat) (mfix : mfixpoint term) (idx : nat),
-          Forall
-            (λ d : def term,
-                expanded Σ (repeat 0 #|mfix| ++ Γ) (dbody d)) mfix 
-        → Forall
-            (λ d : def term,
-                P (repeat 0 #|mfix| ++ Γ) (dbody d)) mfix 
-        → P Γ (tCoFix mfix idx))
-    → (∀ (Γ : list nat) (ind : inductive) 
-         (idx : nat) (mind : mutual_inductive_body) 
-         (idecl : one_inductive_body) 
-         (cname : ident) (c : nat) 
-         (args : list term),
-          declared_constructor Σ (ind, idx) mind idecl (cname, c)
-        → #|args| ≥ ind_npars mind + c
-        → Forall (expanded Σ Γ) args
-        → Forall (P Γ) args
-        → P Γ (mkApps (tConstruct ind idx) args))
-    → (∀ Γ : list nat, P Γ tBox)
-    → ∀ (Γ : list nat) (t : term), expanded Σ Γ t → P Γ t.
-Proof.
-  intros Σ P HRel_app HVar HEvar HLamdba HLetIn HmkApps HConst HCase HProj HFix HCoFix HConstruct HBox.
-  fix f 3.
-  intros Γ t Hexp.  destruct Hexp; eauto.
-  - eapply HRel_app; eauto. clear - f H0. induction H0; econstructor; eauto.
-  - eapply HEvar; eauto. clear - f H. induction H; econstructor; eauto.
-  - eapply HmkApps; eauto. clear - f H0. induction H0; econstructor; eauto.
-  - eapply HCase; eauto. induction H; econstructor; eauto.
-  - assert (Forall (P Γ) args). { clear - H0 f. induction H0; econstructor; eauto. }
-    eapply HFix; eauto.
-    revert H. clear - f.
-    generalize mfix at 1 3. intros mfix0 H.  induction H; econstructor; cbn in *; eauto; split.
-  - eapply HCoFix; eauto.
-    revert H. clear - f.
-    generalize mfix at 1 3. intros mfix0 H.  induction H; econstructor; cbn in *; eauto; split.
-  - eapply HConstruct; eauto.
-    clear - H1 f. induction H1; econstructor; eauto.
-Qed.
-
-
-
-Local Hint Constructors expanded : core.
 
 From MetaCoq.SafeChecker Require Import PCUICWfEnv.
      
 From MetaCoq.Erasure Require Import EAst EAstUtils EInduction EArities Extract Prelim
-    ELiftSubst ESpineView ECSubst.
-
-Hint Rewrite repeat_length : len.
-
-Lemma expanded_closed Σ Γ t : 
-  expanded Σ Γ t -> ELiftSubst.closedn #|Γ| t.
-Proof.
-  induction 1; cbn; eauto.
-  all: try now (rewrite ?closedn_mkApps; rtoProp; repeat solve_all).
-  - rewrite closedn_mkApps. rtoProp. split. cbn.
-    + eapply nth_error_Some_length in H. now eapply Nat.ltb_lt.
-    + solve_all.
-  - rtoProp. repeat split. eauto. solve_all. revert b. now len.
-  - rewrite closedn_mkApps. rtoProp. repeat split; cbn; solve_all.
-    revert  b. now len.
-  - solve_all. revert b. now len.
-Qed.
+    EGlobalEnv ELiftSubst ESpineView ECSubst.
 
 Local Open Scope string_scope.
 Set Asymmetric Patterns.
@@ -227,31 +37,20 @@ Set Warnings "-notation-overridden".
 Import E.
 Set Warnings "+notation-overridden".
 
-Lemma csubst_mkApps {a k f l} : csubst a k (mkApps f l) = mkApps (csubst a k f) (map (csubst a k) l).
-Proof.
-  induction l using rev_ind; simpl; auto.
-  rewrite mkApps_app /= IHl.
-  now rewrite -[EAst.tApp _ _](mkApps_app _ _ [_]) map_app.
-Qed.
+Import MCList (map_InP, map_InP_elim, map_InP_spec).
 
-Equations discr_expanded_head (t : term) : Prop :=
-  discr_expanded_head (tConstruct ind n) := False ;
-  discr_expanded_head (tFix mfix idx) := False ;
-  discr_expanded_head (tRel n) := False ;
-  discr_expanded_head _ := True.
+Equations discr_construct (t : term) : Prop :=
+discr_construct (tConstruct ind n) := False ;
+discr_construct _ := True.
 
-Inductive expanded_head_view : term -> Type :=
-| expanded_head_construct : forall ind n, expanded_head_view (tConstruct ind n)
-| expanded_head_fix : forall mfix idx, expanded_head_view (tFix mfix idx)
-| expanded_head_rel : forall n, expanded_head_view (tRel n)
-| expanded_head_other : forall t, discr_expanded_head t -> expanded_head_view t.
+Inductive construct_view : term -> Type :=
+| view_construct : forall ind n, construct_view (tConstruct ind n)
+| view_other : forall t, discr_construct t -> construct_view t.
 
-Equations expanded_head_viewc t : expanded_head_view t :=
-  expanded_head_viewc (tConstruct ind n) := expanded_head_construct ind n ;
-  expanded_head_viewc (tFix mfix idx) := expanded_head_fix mfix idx ;
-  expanded_head_viewc (tRel n) := expanded_head_rel n ;
-  expanded_head_viewc t := expanded_head_other t I.
-  
+Equations construct_viewc t : construct_view t :=
+construct_viewc (tConstruct ind n) := view_construct ind n ;
+construct_viewc t := view_other t I.
+
 Ltac toAll := 
     repeat match goal with 
       | [ H : forall x, In x ?l -> _ |- _ ] => eapply In_All in H
@@ -261,58 +60,29 @@ Import ECSubst.
 
 Section isEtaExp.
   Context (Σ : global_declarations).
-  Definition lookup_minductive kn : option mutual_inductive_body :=
-    decl <- ETyping.lookup_env Σ kn;; 
-    match decl with
-    | ConstantDecl _ => None
-    | InductiveDecl mdecl => ret mdecl
-    end.
-
-  Definition lookup_inductive kn : option (mutual_inductive_body * one_inductive_body) :=
-    mdecl <- lookup_minductive (inductive_mind kn) ;;
-    idecl <- nth_error mdecl.(ind_bodies) (inductive_ind kn) ;;
-    ret (mdecl, idecl).
-  
-  Definition lookup_inductive_pars kn : option nat := 
-    mdecl <- lookup_minductive kn ;;
-    ret mdecl.(ind_npars).
-  
-  Definition lookup_constructor_pars_args kn c : option (nat * nat) := 
-    '(mdecl, idecl) <- lookup_inductive kn ;;
-    cdecl <- nth_error idecl.(ind_ctors) c ;;
-    ret (mdecl.(ind_npars), cdecl.2).
     
   Definition isEtaExp_app ind c k :=
-    match lookup_constructor_pars_args ind c with
+    match EGlobalEnv.lookup_constructor_pars_args Σ ind c with
     | Some (npars, nargs) => leb (npars + nargs) k
     | None => false
     end.
-
-  Definition isEtaExp_fixapp (mfix : mfixpoint term) idx k :=
-    match nth_error mfix idx with
-    | Some d => Nat.ltb d.(rarg) k
-    | None => false
-    end.    
     
   Import TermSpineView.
 
-  Equations? isEtaExp (Γ : list nat) (e : EAst.term) : bool
+  Equations? isEtaExp (e : EAst.term) : bool
     by wf e (fun x y : EAst.term => size x < size y) :=
-    isEtaExp Γ e with TermSpineView.view e := {
-    | tRel i => option_default (Nat.eqb 0) (nth_error Γ i) false
-    | tEvar ev args => forallb_InP args (fun x H => isEtaExp Γ x)
-    | tLambda na M => isEtaExp (0 :: Γ) M
-    | tApp u v napp nnil with expanded_head_viewc u := 
-      { | expanded_head_construct ind i => isEtaExp_app ind i (List.length v) && forallb_InP v (fun x H => isEtaExp Γ x)
-        | expanded_head_fix mfix idx => isEtaExp_fixapp mfix idx (List.length v) && 
-                                        forallb_InP mfix (fun x H => isEtaExp (rev_map (S ∘ rarg) mfix ++ Γ) x.(dbody)) && forallb_InP v (fun x H => isEtaExp Γ x)
-        | expanded_head_rel n => option_default (fun m => m <=? List.length v) (nth_error Γ n) false && forallb_InP v (fun x H => isEtaExp Γ x) 
-        | expanded_head_other _ _ => isEtaExp Γ u && forallb_InP v (fun x H => isEtaExp Γ x) }
-    | tLetIn na b b' => isEtaExp Γ b && isEtaExp (0 :: Γ) b'
-    | tCase ind c brs => isEtaExp Γ c && forallb_InP brs (fun x H => isEtaExp (repeat 0 #|x.1| ++ Γ) x.2)
-    | tProj p c => isEtaExp Γ c
-    | tFix mfix idx => false
-    | tCoFix mfix idx => forallb_InP mfix (fun x H => isEtaExp (repeat 0 #|mfix| ++ Γ) x.(dbody))
+  | e with TermSpineView.view e := {
+    | tRel i => true
+    | tEvar ev args => forallb_InP args (fun x H => isEtaExp x)
+    | tLambda na M => isEtaExp M
+    | tApp u v napp nnil with construct_viewc u := 
+      { | view_construct ind i => isEtaExp_app ind i (List.length v) && forallb_InP v (fun x H => isEtaExp x)
+        | view_other _ _ => isEtaExp u && forallb_InP v (fun x H => isEtaExp x) }
+    | tLetIn na b b' => isEtaExp b && isEtaExp b'
+    | tCase ind c brs => isEtaExp c && forallb_InP brs (fun x H => isEtaExp x.2)
+    | tProj p c => isEtaExp c
+    | tFix mfix idx => forallb_InP mfix (fun x H => isEtaExp x.(dbody))
+    | tCoFix mfix idx => forallb_InP mfix (fun x H => isEtaExp x.(dbody))
     | tBox => true
     | tVar _ => true
     | tConst _ => true
@@ -323,16 +93,8 @@ Section isEtaExp.
     all:try lia.
     - now apply (In_size id size). 
     - rewrite size_mkApps.
+      change (fun x => size (id x)) with size in H. cbn.
       now apply (In_size id size).
-    - rewrite size_mkApps.
-      apply (In_size id (fun d => size d.(dbody))) in H. unfold id in H. 
-      change (fun x => size x) with size in H. cbn. lia.
-    - rewrite size_mkApps.
-      apply (In_size id size) in H. unfold id in H. 
-      change (fun x => size x) with size in H. cbn. lia.
-    - rewrite size_mkApps.
-      apply (In_size id size) in H. unfold id in H. 
-      change (fun x => size x) with size in H. cbn. lia.
     - now eapply size_mkApps_f.
     - change (fun x => size (id x)) with size in H.
       eapply (In_size id size) in H. unfold id in H.
@@ -351,468 +113,239 @@ Section isEtaExp.
 
   Hint Rewrite @forallb_InP_spec : isEtaExp.
 
-  Lemma isEtaExp_mkApps_nonnil Γ f v :
+
+  Lemma isEtaExp_mkApps_nonnil f v :
     ~~ isApp f -> v <> [] ->
-    isEtaExp Γ (mkApps f v) = match expanded_head_viewc f with 
-      | expanded_head_construct ind i => isEtaExp_app ind i #|v| && forallb (isEtaExp Γ) v
-      | expanded_head_fix mfix idx => isEtaExp_fixapp mfix idx #|v| && forallb (fun x => isEtaExp (rev_map (S ∘ rarg) mfix ++ Γ) x.(dbody)) mfix && forallb (isEtaExp Γ) v
-      | expanded_head_rel n => option_default (fun m => m <=? List.length v) (nth_error Γ n) false && forallb (fun x => isEtaExp Γ x) v
-      | expanded_head_other t discr => isEtaExp Γ f && forallb (isEtaExp Γ) v
+    isEtaExp (mkApps f v) = match construct_viewc f with 
+      | view_construct ind i => isEtaExp_app ind i #|v| && forallb isEtaExp v
+      | view_other t discr => isEtaExp f && forallb isEtaExp v
     end.
   Proof.
     rewrite isEtaExp_equation_1.
     intros napp hv.
     destruct (TermSpineView.view_mkApps (TermSpineView.view (mkApps f v)) napp hv) as [hna [hv' ->]].
-    cbn. destruct (expanded_head_viewc f); cbn; simp isEtaExp => //.
+    cbn. destruct (construct_viewc f); cbn; simp isEtaExp => //.
   Qed.
 
   Tactic Notation "simp_eta" "in" hyp(H) := simp isEtaExp in H; rewrite -?isEtaExp_equation_1 in H.
   Ltac simp_eta := simp isEtaExp; rewrite -?isEtaExp_equation_1.
-
-  Definition is_cons {A} (l : list A) := match l with [] => false | _ => true end.
   
-  Lemma isEtaExp_mkApps Γ f v : ~~ isApp f -> 
-    isEtaExp Γ (mkApps f v) = match expanded_head_viewc f with 
-      | expanded_head_construct ind i => isEtaExp_app ind i #|v| && forallb (isEtaExp Γ) v
-      | expanded_head_fix mfix idx => isEtaExp_fixapp mfix idx #|v| && forallb (fun x => isEtaExp (rev_map (S ∘ rarg) mfix ++ Γ) x.(dbody)) mfix && forallb (isEtaExp Γ) v
-      | expanded_head_rel n => option_default (fun m => m <=? List.length v) (nth_error Γ n) false && forallb (fun x => isEtaExp Γ x) v
-      | expanded_head_other t discr => isEtaExp Γ f && forallb (isEtaExp Γ) v
+  Lemma isEtaExp_mkApps f v : ~~ isApp f ->
+    isEtaExp (mkApps f v) = match construct_viewc f with 
+      | view_construct ind i => isEtaExp_app ind i #|v| && forallb isEtaExp v
+      | view_other t discr => isEtaExp f && forallb isEtaExp v
     end.
   Proof.
     intros napp.
     destruct v using rev_case; simp_eta.
-    - destruct expanded_head_viewc; rewrite ? andb_true_r //. cbn. unfold isEtaExp_fixapp. now destruct (nth_error); cbn.
-      cbn.
-      destruct (nth_error Γ n) as [m | ]; cbn; try reflexivity.
-      destruct (Nat.eqb_spec 0 m), (Nat.leb_spec m 0); try reflexivity; lia.
-    - rewrite isEtaExp_mkApps_nonnil //. destruct v; cbn; try congruence.      
+    - destruct construct_viewc; rewrite andb_true_r //.
+    - rewrite isEtaExp_mkApps_nonnil //. now destruct v; cbn; congruence.
   Qed.
 
-  Lemma isEtaExp_Constructor Γ ind i v :
-    isEtaExp Γ (mkApps (EAst.tConstruct ind i) v) = isEtaExp_app ind i #|v| && forallb (isEtaExp Γ) v.
+  Lemma isEtaExp_Constructor ind i v :
+    isEtaExp (mkApps (EAst.tConstruct ind i) v) = isEtaExp_app ind i #|v| && forallb isEtaExp v.
   Proof.
-    now rewrite isEtaExp_mkApps.
+    rewrite isEtaExp_mkApps //.
   Qed.
- 
-  Lemma isEtaExp_mkApps_intro Γ t l : isEtaExp Γ t -> All (isEtaExp Γ) l -> isEtaExp Γ (mkApps t l).
+
+  Lemma isEtaExp_mkApps_intro t l : isEtaExp t -> All isEtaExp l -> isEtaExp (mkApps t l).
   Proof.
-    revert t Γ; induction l using rev_ind; auto.
-    intros t Γ et a; eapply All_app in a as [].
+    revert t; induction l using rev_ind; auto.
+    intros t et a; eapply All_app in a as [].
     depelim a0. clear a0.
     destruct (decompose_app t) eqn:da.
     rewrite (decompose_app_inv da) in et *.
     pose proof (decompose_app_notApp _ _ _ da).
     destruct l0. simp_eta.
     - rewrite isEtaExp_mkApps //.
-      destruct expanded_head_viewc.
-      + cbn. len.
-        rtoProp; repeat solve_all. cbn in et. simp isEtaExp in et.
-        eapply isEtaExp_app_mon; tea; lia. 
-        eapply All_app_inv; eauto.
-      + cbn in *; congruence.
-      + simp_eta in et.
-       destruct (nth_error Γ n) as [m | ] eqn:Heq; cbn in et; try eauto.
-        eapply Nat.eqb_eq in et. rewrite <- et.
-        rtoProp. split. cbn. eauto.
-        solve_all. eapply All_app_inv; solve_all.
-      + rewrite et forallb_app /=. rtoProp; repeat solve_all. 
+      destruct construct_viewc. cbn. len.
+      rtoProp; repeat solve_all. cbn in et. simp isEtaExp in et.
+      eapply isEtaExp_app_mon; tea; lia.
+      eapply All_app_inv; eauto. rewrite et forallb_app /=.
+      rtoProp; repeat solve_all.
     - rewrite isEtaExp_mkApps in et => //.
-      destruct expanded_head_viewc.
-      + rewrite -mkApps_app. rewrite isEtaExp_Constructor.
-        cbn. cbn. rtoProp; solve_all.
-        eapply isEtaExp_app_mon; tea. cbn. len. lia. now depelim H1.
-        depelim H1. solve_all. eapply All_app_inv => //.
-        eapply All_app_inv => //. eauto.
-      + rewrite -mkApps_app. rewrite isEtaExp_mkApps //. simp expanded_head_viewc.
-        rewrite /isEtaExp_fixapp in et |- *.
-        rtoProp; repeat split.
-        * destruct nth_error; try congruence. eapply Nat.ltb_lt. eapply Nat.ltb_lt in H0.
-          cbn in H0. len. lia.
-        * solve_all.
-        * solve_all. eapply All_app_inv; solve_all. eapply All_app_inv; solve_all.
-      + rewrite -mkApps_app. rewrite isEtaExp_mkApps //.
-        cbn [expanded_head_viewc]. rtoProp. split.
-        destruct (nth_error Γ n) as [m | ] eqn:Heq; cbn in H0; eauto.
-        cbn. eapply Nat.leb_le in H0. eapply Nat.leb_le. revert H0. len. lia.
-        solve_all. eapply All_app_inv. 2: eapply All_app_inv. all: solve_all.
-      + rewrite -mkApps_app. rewrite isEtaExp_mkApps //.
-        destruct (expanded_head_viewc t0) => //.
-        move/andP: et => [] -> /=. rtoProp; solve_all.
-        rewrite forallb_app. rtoProp; repeat solve_all.
-        eapply All_app_inv; eauto.
+      destruct construct_viewc.
+      rewrite -mkApps_app. rewrite isEtaExp_Constructor.
+      cbn. cbn. rtoProp; solve_all.
+      eapply isEtaExp_app_mon; tea. cbn. len. lia. now depelim H1.
+      depelim H1. solve_all. eapply All_app_inv => //.
+      eapply All_app_inv => //. eauto.
+      rewrite -mkApps_app. rewrite isEtaExp_mkApps //.
+      destruct (construct_viewc t0) => //.
+      move/andP: et => [] -> /=. rtoProp; solve_all.
+      rewrite forallb_app. rtoProp; repeat solve_all.
+      eapply All_app_inv; eauto.
   Qed.
 
-  Hint Rewrite repeat_length : len.
-
-  Lemma nth_error_app_Some {X} (A B : list X) n x : 
-    nth_error A n = Some x -> nth_error (A ++ B) n = Some x.
+  Lemma etaExp_csubst a k b : 
+    isEtaExp a -> isEtaExp b -> isEtaExp (ECSubst.csubst a k b).
   Proof.
-    induction n in A |- *; destruct A; cbn; try congruence.
-    eauto.
-  Qed.
-
-  Lemma expanded_weakening Γ' Γ t :
-    isEtaExp Γ t ->
-    isEtaExp (Γ ++ Γ') t.
-  Proof.
-    funelim (isEtaExp Γ t); simp_eta; eauto; intros Hexp; toAll; solve_all; rtoProp; repeat solve_all; eauto.
-    - destruct nth_error eqn:E; try easy. erewrite nth_error_app_Some; eauto.
-    - rewrite app_assoc. eapply a, b. reflexivity.
-    - rewrite app_assoc. eapply a, b. reflexivity.
-    - rewrite isEtaExp_mkApps => //. cbn [expanded_head_viewc]. rtoProp; repeat solve_all.
-    - rewrite isEtaExp_mkApps => //. cbn [expanded_head_viewc]. rtoProp; repeat solve_all.
-      rewrite app_assoc. eapply a, b. reflexivity.
-    - rewrite isEtaExp_mkApps => //. cbn [expanded_head_viewc]. rtoProp; repeat solve_all.
-      destruct nth_error eqn:E; try easy. erewrite nth_error_app_Some; eauto.
-    - rewrite isEtaExp_mkApps => //. rewrite Heq. rtoProp; repeat solve_all.
-  Qed.
-
-(*   Lemma expanded_lift Γ' Γ'' Γ t :
-    isEtaExp (Γ' ++ Γ)%list t ->
-    isEtaExp (Γ' ++ Γ'' ++ Γ)%list (lift #|Γ''| #|Γ'| t).
-  Proof.
-  Admitted.
- *)
-  Lemma isEtaExp_closed Γ t : 
-    isEtaExp Γ t -> closedn #|Γ| t.
-  Proof.
-    funelim (isEtaExp Γ t); simp_eta; cbn [closedn];
-    rewrite ?closedn_mkApps; rtoProp; (try toAll); repeat solve_all.
-    - destruct nth_error eqn:Hn; cbn in H; try easy.
-      eapply nth_error_Some_length in Hn. now eapply Nat.ltb_lt.
-    - eapply a in b. 2: f_equal. revert b. now len.
-    - easy.
-    - eapply a in b. 2: f_equal. revert b. now len.
-    - cbn. solve_all. eapply a in b. 2: reflexivity. revert b. now len.
-    - destruct nth_error eqn:Hn; cbn in H1; try easy.
-      eapply nth_error_Some_length in Hn. now eapply Nat.ltb_lt.
-  Qed.
-
-  Lemma etaExp_csubst' a k b n Γ Δ : 
-    #|Γ| = k ->
-    isEtaExp [] a -> isEtaExp (Γ ++ [n] ++ Δ) b -> isEtaExp (Γ ++ Δ) (ECSubst.csubst a k b).
-  Proof.
-    intros Hk H.
-    assert (Hcl : closed a) by now eapply isEtaExp_closed in H. revert H.
-    remember (Γ ++ [n] ++ Δ)%list as Γ_.
-    funelim (isEtaExp Γ_ b); try simp_eta; eauto; try fold csubst;
-      try toAll; repeat solve_all; subst.
-    - intros. simp isEtaExp ; cbn. destruct (Nat.compare_spec #|Γ0| i) => //; simp_eta.
-      + eapply expanded_weakening with (Γ := []). eauto.
-      + rewrite nth_error_app2. lia.
-        rewrite !nth_error_app2 in H0. lia. cbn. lia.
-        erewrite option_default_ext; eauto.
-        f_equal. destruct i; cbn; lia.
-      + now rewrite !nth_error_app1 in H0 |- *; try lia.
-    - eapply H with (Γ := 0 :: Γ0); cbn; eauto.
-    - move/andP: H2 => [] etab etab'. simp_eta.
+    funelim (isEtaExp b); try simp_eta; eauto;
+      try toAll; repeat solve_all.
+    - intros. simp isEtaExp ; cbn. destruct Nat.compare => //. simp_eta in H.
+    - move/andP: H2 => [] etab etab'.
       apply/andP. split; eauto.
-      eapply H0 with (Γ := 0 :: Γ0); cbn; eauto.
     - rtoProp. intuition eauto.
-      solve_all. rewrite app_assoc. eapply a0; cbn; eauto. now len. cbn.
-      now rewrite app_assoc.
-    - rewrite app_assoc. eapply a0; len; eauto. now rewrite app_assoc.
-    - fold csubst. move/andP: H1 => [] etaexp h.
+      solve_all.
+    - move/andP: H1 => [] etaexp h.
       rewrite csubst_mkApps /=.
       rewrite isEtaExp_Constructor. solve_all.
       rewrite map_length. rtoProp; solve_all. solve_all.
     - rewrite csubst_mkApps /=.
-      move/andP : H2 => [] /andP [] eu ef ev.
-      rewrite isEtaExp_mkApps //.
-      simp expanded_head_viewc.
-      rtoProp; repeat split.
-      + rewrite /isEtaExp_fixapp in eu |- *. rewrite nth_error_map. destruct nth_error; try congruence.
-        cbn. now len.
-      + solve_all.
-        rewrite app_assoc.  eapply a0; len; eauto. cbn. f_equal.
-        rewrite app_assoc. do 2 f_equal.
-        rewrite !rev_map_spec. f_equal. rewrite map_map. now eapply map_ext.      
-      + solve_all.
-    - rewrite csubst_mkApps /=. rtoProp. destruct (Nat.compare_spec #|Γ0| n) => //; simp_eta.
-      + eapply isEtaExp_mkApps_intro => //. 2: solve_all.
-        now eapply expanded_weakening with (Γ := []).
-      + rewrite isEtaExp_mkApps; eauto. cbn [expanded_head_viewc].
-        rtoProp. split. 2: solve_all.
-        rewrite !nth_error_app2 in H1 |- *; cbn; try lia.
-        len. erewrite option_default_ext; eauto. f_equal.
-        destruct n; cbn; lia.
-      + rewrite isEtaExp_mkApps; eauto. cbn [expanded_head_viewc].
-        rtoProp. split. 2: solve_all. len. now rewrite !nth_error_app1 in H1 |- *; try lia.
-    - rewrite csubst_mkApps /=.
       move/andP: H2 => [] eu ev.
-      eapply isEtaExp_mkApps_intro => //. 2: solve_all.
-      eauto. 
-  Qed.
-
-  Lemma etaExp_csubst a b n : 
-    isEtaExp []a -> isEtaExp [n] b -> isEtaExp [] (ECSubst.csubst a 0 b).
-  Proof.
-    intros.
-    eapply etaExp_csubst' with (Γ := []); eauto.
-  Qed.
-
-  Lemma etaExp_fixsubst k b Γ Δ mfix idx d : 
-    #|Γ| = k ->
-    nth_error mfix idx = Some d ->
-    closed (EAst.tFix mfix idx) ->
-    forallb (fun x => isEtaExp (rev_map (S ∘ rarg) mfix) x.(dbody)) mfix ->
-    isEtaExp (Γ ++ [1 + d.(EAst.rarg)] ++ Δ) b -> isEtaExp (Γ ++ Δ) (ECSubst.csubst (EAst.tFix mfix idx) k b).
-  Proof.
-    intros Hk Hnth Hcl. 
-    remember (Γ ++ [1 + d.(EAst.rarg)] ++ Δ)%list as Γ_.
-    funelim (isEtaExp Γ_ b); try simp_eta; eauto; try fold csubst;
-      try toAll; try now repeat solve_all; subst.
-    - intros. simp isEtaExp ; cbn. destruct (Nat.compare_spec #|Γ0| i) => //; simp_eta.
-      + rewrite nth_error_app2 in H0; try lia; cbn in H0; try easy. subst. rewrite minus_diag in H0. cbn in H0. easy.
-      + rewrite !nth_error_app2 in H0 |- *; cbn; try lia.
-        erewrite option_default_ext; eauto. f_equal.
-        destruct i; cbn; lia.
-      + now rewrite !nth_error_app1 in H0 |- *; try lia.
-    - intros. solve_all. eapply a; eauto. solve_all.
-    - eapply H with (Γ := 0 :: Γ0); cbn -[isEtaExp]; eauto. 
-    - solve_all. move/andP: H2 => [] etab etab'. simp_eta.
-      apply/andP. split; eauto.
-      eapply H0 with (Γ := 0 :: Γ0); cbn; eauto.
-    - solve_all. rtoProp. intuition eauto.
-      solve_all. rewrite app_assoc. eapply a; cbn-[isEtaExp]; eauto. now len. cbn.
-      now rewrite app_assoc.
-      solve_all.
-    - solve_all. rewrite app_assoc. solve_all.  eapply a; len; eauto.
-      { cbn in Hcl. solve_all. rewrite Nat.add_0_r in a0. eauto. }
-      now rewrite app_assoc.
-      solve_all.
-    - solve_all. fold csubst. move/andP: H1 => [] etaexp h.
-      rewrite csubst_mkApps /=.
-      rewrite isEtaExp_Constructor. solve_all.
-      rewrite map_length. rtoProp; solve_all.
-      solve_all.
-      eapply a; eauto.
-      solve_all.
-    - solve_all. rewrite csubst_mkApps /=.
-      move/andP : H2 => [] /andP [] eu ef ev.
-      rewrite isEtaExp_mkApps //.
-      simp expanded_head_viewc.
-      rtoProp; repeat split.
-      + rewrite /isEtaExp_fixapp in eu |- *. rewrite nth_error_map.
-        destruct (nth_error mfix idx); try congruence.
-        cbn. now len.
-      + solve_all.
-        rewrite app_assoc.  eapply a; len; eauto.
-        { cbn in Hcl. solve_all. rewrite Nat.add_0_r in a0. eauto. }
-        cbn. f_equal.
-        rewrite app_assoc. do 2 f_equal.
-        rewrite !rev_map_spec. f_equal. rewrite map_map. now eapply map_ext.
-        solve_all.      
-      + solve_all. eapply a; eauto. solve_all.
-    - rewrite csubst_mkApps /=. rtoProp. destruct (Nat.compare_spec #|Γ0| n) => //; simp_eta.
-      + rewrite isEtaExp_mkApps => //. cbn [expanded_head_viewc].
-        rtoProp. repeat split; eauto.
-        * unfold isEtaExp_fixapp. rewrite Hnth. len. destruct H2 as [Hn H2].
-          subst. rewrite nth_error_app2 in Hn; try lia.
-          rewrite minus_diag in Hn. cbn in Hn. eapply Nat.ltb_lt.
-          eapply Nat.leb_le in Hn. lia.        
-        * cbn in Hcl. solve_all.
-          now eapply expanded_weakening.
-        * destruct H2. solve_all. eapply a ;eauto. solve_all.          
-      + rewrite isEtaExp_mkApps; eauto. cbn [expanded_head_viewc].
-        rtoProp. intros. destruct H2. split. 2:{ solve_all. eapply a; eauto. solve_all. }
-        rewrite !nth_error_app2 in H2 |- *; try lia.
-        rewrite (nth_error_app2 ([S (EAst.rarg d)])) in H2; cbn; try lia.
-        len.
-        erewrite option_default_ext. eauto. f_equal.
-        destruct n; cbn; lia.
-      + rewrite isEtaExp_mkApps; eauto. cbn [expanded_head_viewc].
-        intros. destruct H2.
-        rtoProp. split. 2:{ solve_all. eapply a; eauto. solve_all. }
-        len.
-        now rewrite !nth_error_app1 in H2 |- *; try lia.
-    - intros. rtoProp. rewrite csubst_mkApps /=.
-      eapply isEtaExp_mkApps_intro => //. 2:{ solve_all. eapply a; eauto. solve_all. }
-      eapply H; eauto.
+      specialize (H _ k H1 eu).
+      eapply isEtaExp_mkApps_intro => //. solve_all.
   Qed.
   
-  Lemma isEtaExp_substl Γ Δ s t : 
-    #|Γ| = #|s| ->
-    forallb (isEtaExp []) s -> isEtaExp (Γ ++ Δ) t ->
-    isEtaExp Δ (substl s t).
+  Lemma isEtaExp_substl s t : 
+    forallb isEtaExp s -> isEtaExp t ->
+    isEtaExp (substl s t).
   Proof.
-    induction s in Γ, t |- *; simpl; auto;
-    rtoProp; intuition eauto using etaExp_csubst.
-    - destruct Γ; eauto; cbn in *; lia.
-    - destruct Γ; cbn in H; invs H.
-      eapply IHs; eauto. eapply etaExp_csubst' with (Γ := []); eauto.
-  Qed.
-
-  Lemma isEtaExp_fixsubstl Δ mfix t : 
-    forallb (fun x => isEtaExp (rev_map (S ∘ rarg) mfix) x.(dbody)) mfix ->
-    isEtaExp ((rev_map (S ∘ rarg) mfix) ++ Δ) t ->
-    isEtaExp Δ (substl (fix_subst mfix) t).
-  Proof.
-    intros Hall Heta.
-    assert (Hcl : closed (EAst.tFix mfix 0) ). { cbn. solve_all. eapply isEtaExp_closed in H. revert H. now len. }
-    revert Hcl Hall Heta.  
-    intros Hcl Hall Heta.
-    cbn in Hcl. solve_all.
-    unfold fix_subst.
-    revert Hall Heta.
-  
-    generalize (@eq_refl _ mfix).
-    setoid_rewrite <- app_nil_r at 1.
-    generalize ((@nil (EAst.def EAst.term))).
-    generalize (mfix) at 1 6 8.
-    
-    intros mfix0. revert mfix Δ t.
-    induction mfix0  using rev_ind; intros.
-    - cbn -[isEtaExp] in *. eauto.
-    - cbn -[isEtaExp] in *. rewrite app_length Nat.add_comm. cbn -[substl isEtaExp].
-      eapply IHmfix0. 
-      + subst. now rewrite <- app_assoc.
-      + solve_all.
-      + eapply etaExp_fixsubst with (Γ := []); eauto.
-        2: cbn; solve_all. 2: solve_all.
-        2:{ cbn -[isEtaExp] in *. revert Heta.
-            rewrite !rev_map_spec map_app rev_app_distr. cbn -[isEtaExp] in *. intros.
-            exact Heta.
-        }
-        subst. rewrite <- app_assoc. cbn. now eapply nth_error_snoc.
+    induction s in t |- *; simpl; auto. rtoProp; intuition eauto using etaExp_csubst.
   Qed.
 
   Lemma isEtaExp_iota_red pars args br :
-    Forall (closedn 0) args ->
-    forallb (isEtaExp []) args ->
-    isEtaExp (repeat 0 (#|args| - pars)) br.2 ->
-    isEtaExp [] (ETyping.iota_red pars args br).
+    forallb isEtaExp args ->
+    isEtaExp br.2 ->
+    isEtaExp (EGlobalEnv.iota_red pars args br).
   Proof.
-    intros  Hcl etaargs etabr.
-    unfold ETyping.iota_red.
-    erewrite (isEtaExp_substl _ []); eauto.
-    - shelve.
-    - solve_all. eapply All_skipn. solve_all.
-    - rewrite app_nil_r. eauto.
-    Unshelve. len. now rewrite List.skipn_length.  
+    intros etaargs etabr.
+    unfold EGlobalEnv.iota_red.
+    rewrite isEtaExp_substl // forallb_rev forallb_skipn //.
   Qed.
-   
-(*
-
+  
   Lemma isEtaExp_fix_subst mfix : 
-    forallb (isEtaExp (repeat 0 #|mfix|) ∘ dbody) mfix ->
-    forallb (isEtaExp []) (ETyping.fix_subst mfix).
+    forallb (isEtaExp ∘ dbody) mfix ->
+    forallb isEtaExp (EGlobalEnv.fix_subst mfix).
   Proof.
-    unfold ETyping.fix_subst.
-    generalize (@eq_refl _ #|mfix|). 
-    generalize #|mfix| at 1 3 4.
-    intros. solve_all. revert n H H0.
+    unfold EGlobalEnv.fix_subst. generalize #|mfix|.
+    solve_all. solve_all. revert n.
     induction n; intros; simp_eta; constructor; auto.
-    + simp_eta.
-    simp isEtaExp. solve_all. 
-  Qed. 
+    simp isEtaExp. solve_all.
+  Qed.
 
-  *)
- 
   Lemma isEtaExp_cofix_subst mfix : 
-    forallb (isEtaExp (repeat 0 #|mfix|) ∘ dbody) mfix ->
-    forallb (isEtaExp []) (ETyping.cofix_subst mfix).
+    forallb (isEtaExp ∘ dbody) mfix ->
+    forallb isEtaExp (EGlobalEnv.cofix_subst mfix).
   Proof.
-    intros. solve_all.
-    unfold ETyping.cofix_subst.
-    unfold cofix_subst. generalize #|mfix|. intros n. solve_all. induction n.
-      + econstructor.
-      + econstructor. simp_eta. solve_all. now rewrite app_nil_r. solve_all.
-  Qed. 
+    unfold EGlobalEnv.cofix_subst. generalize #|mfix|.
+    solve_all. solve_all. revert n.
+    induction n; intros; simp_eta; constructor; auto.
+    simp isEtaExp. solve_all.
+  Qed.
   
   Lemma isEtaExp_cunfold_fix mfix idx n f : 
-    forallb (isEtaExp (rev_map (S ∘ rarg) mfix) ∘ dbody) mfix ->
+    forallb (isEtaExp ∘ dbody) mfix ->
     Ee.cunfold_fix mfix idx = Some (n, f) ->
-    isEtaExp [] f.
+    isEtaExp f.
   Proof.
     intros heta.
     unfold Ee.cunfold_fix.
     destruct nth_error eqn:heq => //.
     intros [= <- <-] => /=.
-    eapply isEtaExp_fixsubstl.
-    - solve_all.
-    - rewrite app_nil_r. solve_all. eapply All_nth_error in heta; eauto.
+    apply isEtaExp_substl.
+    now apply isEtaExp_fix_subst.
+    eapply forallb_nth_error in heta; tea.
+    now erewrite heq in heta.
   Qed.
   
   Lemma isEtaExp_cunfold_cofix mfix idx n f : 
-    forallb (isEtaExp (repeat 0 #|mfix|) ∘ dbody) mfix ->
+    forallb (isEtaExp ∘ dbody) mfix ->
     Ee.cunfold_cofix mfix idx = Some (n, f) ->
-    isEtaExp [] f.
+    isEtaExp f.
   Proof.
     intros heta.
     unfold Ee.cunfold_cofix.
     destruct nth_error eqn:heq => //.
     intros [= <- <-] => /=.
-    eapply isEtaExp_substl.
-    3:{ solve_all. eapply nth_error_all in heta; eauto. rewrite app_nil_r. eapply heta. }
-    - len. now rewrite cofix_subst_length.
-    - solve_all. unfold cofix_subst. generalize #|mfix|. clear - heta. induction n; econstructor; eauto.
-      simp_eta. solve_all. now rewrite app_nil_r.
-  Qed.
-
-  Lemma isEtaExp_tApp Γ f u : isEtaExp Γ (mkApps f u) -> 
-    let (hd, v) := decompose_app (mkApps f u) in
-    match expanded_head_viewc hd with
-      | expanded_head_construct ind i => isEtaExp_app ind i #|v| && forallb (isEtaExp Γ) v
-      | expanded_head_fix mfix idx => isEtaExp_fixapp mfix idx #|v| && forallb (fun x => isEtaExp (rev_map (S ∘ rarg) mfix ++ Γ) x.(dbody)) mfix && forallb (isEtaExp Γ) v
-      | expanded_head_rel n => (option_default (fun m => m <=? List.length v) (nth_error Γ n) false) && forallb (fun x => isEtaExp Γ x) v
-      | expanded_head_other t discr => isEtaExp Γ hd && forallb (isEtaExp Γ) v
-      end. (* 
-    | expanded_head_construct kn c => isEtaExp_app Σ kn c #|args| && forallb (isEtaExp Σ) args
-    | expanded_head_fix mfix idx => isEtaExp_fixapp mfix idx #|args| && forallb mfix (fun x => isEtaExp Σ x.(dbody)) && forallb (isEtaExp Σ) args
-    | expanded_head_rel n => (nth n Γ 0 <=? List.length v) && forallb (fun x => isEtaExp Γ x) v
-    | expanded_head_other u discr => isEtaExp Σ hd && forallb (isEtaExp Σ) args
-    end. *)
-  Proof.
-    destruct decompose_app eqn:da.
-    rewrite (decompose_app_inv da).
-    pose proof (decompose_app_notApp _ _ _ da).
-    intros eq.
-    rewrite isEtaExp_mkApps in eq; eauto.
+    apply isEtaExp_substl.
+    now apply isEtaExp_cofix_subst.
+    eapply forallb_nth_error in heta; tea.
+    now erewrite heq in heta.
   Qed.
 
 End isEtaExp.
 Global Hint Rewrite @forallb_InP_spec : isEtaExp.
 
-Module GlobalContextMap.
-  Record t := 
-  { global_decls :> global_declarations; 
-    map : EnvMap.t global_decl;
-    repr : EnvMap.repr global_decls map;
-    wf : EnvMap.fresh_globals global_decls }.
-  
-  Definition lookup_minductive Σ kn : option mutual_inductive_body :=
-    decl <- EnvMap.lookup kn Σ.(map);; 
-    match decl with
-    | ConstantDecl _ => None
-    | InductiveDecl mdecl => ret mdecl
-    end.
+From MetaCoq.Template Require Import config utils BasicAst Universes.
+From MetaCoq.Erasure Require Import EAst EGlobalEnv EAstUtils.
 
-  Definition lookup_inductive Σ kn : option (mutual_inductive_body * one_inductive_body) :=
-    mdecl <- lookup_minductive Σ (inductive_mind kn) ;;
-    idecl <- nth_error mdecl.(ind_bodies) (inductive_ind kn) ;;
-    ret (mdecl, idecl).
-  
-  Definition lookup_inductive_pars Σ kn : option nat := 
-    mdecl <- lookup_minductive Σ kn ;;
-    ret mdecl.(ind_npars).
+Section expanded.
 
-  Lemma lookup_inductive_pars_spec Σ kn : lookup_inductive_pars Σ kn = EEtaExpanded.lookup_inductive_pars Σ kn.
-  Proof.
-    rewrite /lookup_inductive_pars /EEtaExpanded.lookup_inductive_pars.
-    rewrite /lookup_inductive /EEtaExpanded.lookup_inductive.
-    rewrite /lookup_minductive /EEtaExpanded.lookup_minductive.
-    rewrite (EnvMap.lookup_spec Σ.(global_decls)).
-    eapply wf. eapply repr. reflexivity.
-  Qed.
+Variable Σ : global_declarations.
 
-  Program Definition make (g : global_declarations) (Hg : EnvMap.fresh_globals g): t :=
-    {| global_decls := g;
-       map := EnvMap.of_global_env g |}.
+Local Unset Elimination Schemes.
 
-End GlobalContextMap.
-Coercion GlobalContextMap.global_decls : GlobalContextMap.t >-> global_declarations.
+Inductive expanded : term -> Prop :=
+| expanded_tRel (n : nat) : expanded (tRel n)
+| expanded_tVar (id : ident) : expanded (tVar id)
+| expanded_tEvar (ev : nat) (args : list term) : Forall expanded args -> expanded (tEvar ev args)
+| expanded_tLambda (na : name) (body : term) : expanded body -> expanded (tLambda na body)
+| expanded_tLetIn (na : name) (def : term)(body : term) : expanded def -> expanded body -> expanded (tLetIn na def body)
+| expanded_mkApps (f : term) (args : list term) : ~ isConstruct f -> expanded f -> Forall expanded args -> expanded (mkApps f args)
+| expanded_tConst (c : kername) : expanded (tConst c)
+| expanded_tCase (ind : inductive) (pars : nat) (discr : term) (branches : list (list name × term)) : 
+    expanded discr -> Forall (fun br => expanded br.2) branches -> expanded (tCase (ind, pars) discr branches)
+| expanded_tProj (proj : projection) (t : term) : expanded t -> expanded (tProj proj t)
+| expanded_tFix (mfix : mfixpoint term) (idx : nat) :  Forall (fun d => expanded d.(dbody)) mfix -> expanded (tFix mfix idx)
+| expanded_tCoFix (mfix : mfixpoint term) (idx : nat) : Forall (fun d => expanded d.(dbody)) mfix -> expanded (tCoFix mfix idx)
+| expanded_tConstruct_app ind idx mind idecl cname c args :
+    declared_constructor Σ (ind, idx) mind idecl (cname, c) ->
+    #|args| >= ind_npars mind + c -> 
+    Forall expanded args ->
+    expanded (mkApps (tConstruct ind idx) args)
+| expanded_tBox : expanded tBox.
 
+End expanded.
+
+Lemma expanded_ind :
+forall (Σ : global_declarations) (P : term -> Prop),
+(forall n : nat, P (tRel n)) ->
+(forall id : ident, P (tVar id)) ->
+(forall (ev : nat) (args : list term), Forall (expanded Σ) args -> Forall P args -> P (tEvar ev args)) ->
+(forall (na : name) (body : term),
+ expanded Σ body -> P body -> P (tLambda na body)) ->
+(forall (na : name) (def body : term),
+ expanded Σ def ->
+ P def -> expanded Σ body -> P body -> P (tLetIn na def body)) ->
+(forall (f4 : term) (args : list term),
+ ~ isConstruct f4 ->
+ expanded Σ f4 -> P f4 -> Forall (expanded Σ) args -> Forall P args -> P (mkApps f4 args)) ->
+(forall c : kername, P (tConst c)) ->
+(forall (ind : inductive) (pars : nat) (discr : term)
+   (branches : list (list name × term)),
+ expanded Σ discr ->
+ P discr ->
+ Forall (fun br : list name × term => expanded Σ br.2) branches ->
+ Forall (fun br : list name × term => P br.2) branches ->
+ P (tCase (ind, pars) discr branches)) ->
+(forall (proj : projection) (t : term),
+ expanded Σ t -> P t -> P (tProj proj t)) ->
+(forall (mfix : mfixpoint term) (idx : nat),
+ Forall (fun d : def term => expanded Σ (dbody d)) mfix ->  Forall (fun d : def term => P (dbody d)) mfix  -> P (tFix mfix idx)) ->
+(forall (mfix : mfixpoint term) (idx : nat),
+ Forall (fun d : def term => expanded Σ (dbody d)) mfix ->  Forall (fun d : def term => P (dbody d)) mfix ->
+ P (tCoFix mfix idx)) ->
+(forall (ind : inductive) (idx : nat) (mind : mutual_inductive_body)
+   (idecl : one_inductive_body) (cname : ident) (c : nat) 
+   (args : list term),
+ declared_constructor Σ (ind, idx) mind idecl (cname, c) ->
+ #|args| >= ind_npars mind + c -> Forall (expanded Σ) args -> Forall P args -> P (mkApps (tConstruct ind idx) args)) ->
+(P tBox) ->
+forall t : term, expanded Σ t -> P t.
+Proof. 
+  intros. revert t H12.
+  fix f 2.
+  intros t Hexp. destruct Hexp; eauto.
+  - eapply H1; eauto. induction H12; econstructor; cbn in *; eauto.
+  - eapply H4; eauto. induction H13; econstructor; cbn in *; eauto.
+  - eapply H6; eauto. induction H12; econstructor; cbn in *; eauto.
+  - eapply H8; eauto. induction H12; econstructor; cbn in *; eauto.
+  - eapply H9; eauto. induction H12; econstructor; cbn in *; eauto.
+  - eapply H10; eauto. clear - H14 f. induction H14; econstructor; cbn in *; eauto.
+Qed.
+
+Local Hint Constructors expanded : core .
 Tactic Notation "simp_eta" "in" hyp(H) := simp isEtaExp in H; rewrite -?isEtaExp_equation_1 in H.
 Ltac simp_eta := simp isEtaExp; rewrite -?isEtaExp_equation_1.
 
@@ -841,34 +374,26 @@ Proof.
   intros. eapply isEtaExp_app_expanded. eauto 8.
 Qed.
 
-Lemma isEtaExp_expanded Σ Γ t :
-  isEtaExp Σ Γ t -> expanded Σ Γ t.
+Lemma isEtaExp_expanded Σ t :
+  isEtaExp Σ t -> expanded Σ t.
 Proof.
-  funelim (isEtaExp Σ Γ t); intros; solve_all; eauto.
-  - eapply expanded_tRel_app with (args := []). destruct (nth_error); invs H. f_equal. eapply Nat.eqb_eq in H1; eauto. cbn. lia. econstructor.
-  - rewrite forallb_InP_spec in H0. eapply forallb_Forall in H0. eapply In_All in H. econstructor. solve_all.
+  funelim (isEtaExp Σ t); intros; solve_all; eauto.
+  - rewrite forallb_InP_spec in H0. eapply forallb_Forall in H0. eapply In_All in H.
+    econstructor. solve_all.
   - eapply andb_true_iff in H1 as []; eauto.
   - eapply isEtaExp_app_expanded in H as (? & ? & ? & ? & ? & ?).
     eapply expanded_tConstruct_app with (args := []); eauto.
   - eapply andb_true_iff in H1 as []. destruct ind. econstructor; eauto.
     rewrite forallb_InP_spec in H2. eapply forallb_Forall in H2. 
     eapply In_All in H0. solve_all.
-  - congruence.
+  - econstructor. rewrite forallb_InP_spec in H0. eapply forallb_Forall in H0. 
+    eapply In_All in H. solve_all.
   - econstructor. rewrite forallb_InP_spec in H0. eapply forallb_Forall in H0. 
     eapply In_All in H. solve_all.
   - eapply andb_true_iff in H0 as []. eapply In_All in H.
     rewrite forallb_InP_spec in H1. eapply forallb_Forall in H1.
     eapply isEtaExp_app_expanded in H0 as (? & ? & ? & ? & ? & ?).
     eapply expanded_tConstruct_app; eauto. solve_all.
-  - rtoProp. rewrite forallb_InP_spec in H2. rewrite forallb_InP_spec in H3. eapply In_All in H. eapply In_All in H0. 
-    unfold isEtaExp_fixapp in H1. destruct nth_error eqn:E; try congruence.
-    eapply expanded_tFix.
-    all: try now solve_all.
-    eapply Nat.ltb_lt in H1. lia.
-  - rtoProp. destruct (nth_error) eqn:Hn; invs H0.
-    econstructor. eauto. eapply Nat.leb_le; eauto.  rewrite forallb_InP_spec in H1.
-    eapply Forall_forall. solve_all. eapply H; eauto.
-    eapply All_Forall, Forall_forall in H1; eauto.
   - eapply andb_true_iff in H1 as []. rewrite forallb_InP_spec in H2. eapply forallb_Forall in H2.
     econstructor.
     + destruct u; inv Heq; eauto.
@@ -876,552 +401,16 @@ Proof.
     + eapply In_All in H0. solve_all.
 Qed.
 
-Lemma expanded_isEtaExp Σ Γ t :
-  expanded Σ Γ t -> isEtaExp Σ Γ t.
+Lemma expanded_isEtaExp Σ t :
+  expanded Σ t -> isEtaExp Σ t.
 Proof.
   induction 1; simp_eta; eauto.
   all: try now (
     (try (eapply andb_true_iff; split; eauto));
     (try eapply forallb_Forall); 
     eauto).
-  - rewrite isEtaExp_mkApps //. cbn [expanded_head_viewc].
-    rtoProp. split. 2: solve_all. rewrite H.  now eapply Nat.leb_le.
-  - eapply isEtaExp_mkApps_intro; eauto. solve_all. 
-  - rewrite isEtaExp_mkApps //. cbn [expanded_head_viewc]. rtoProp. repeat split.
-    + unfold isEtaExp_fixapp. rewrite H4. eapply Nat.ltb_lt. lia.
-    + solve_all.
-    + solve_all.
+  - eapply isEtaExp_mkApps_intro; eauto. solve_all.
   - rewrite isEtaExp_Constructor. eapply andb_true_iff.
     split. 2: eapply forallb_Forall.
     2: solve_all. eapply expanded_isEtaExp_app_; eauto.
 Qed.
-
-Definition isEtaExp_constant_decl Σ cb := 
-  option_default (isEtaExp Σ []) cb.(cst_body) true.
-
-Definition isEtaExp_decl Σ d :=
-  match d with
-  | ConstantDecl cb => isEtaExp_constant_decl Σ cb
-  | InductiveDecl idecl => true
-  end.
-
-Fixpoint isEtaExp_env (Σ : global_declarations) := 
-  match Σ with 
-  | [] => true
-  | decl :: Σ => isEtaExp_decl Σ decl.2 && isEtaExp_env Σ
-  end.
-
-Lemma closedn_mkApps k f l : closedn k (mkApps f l) = closedn k f && forallb (closedn k) l.
-Proof.
-  induction l in f |- *; cbn; auto.
-  - now rewrite andb_true_r.
-  - now rewrite IHl /= andb_assoc.
-Qed.
-
-Lemma lookup_inductive_pars_constructor_pars_args Σ {ind n pars args} : 
-  lookup_constructor_pars_args Σ ind n = Some (pars, args) ->
-  lookup_inductive_pars Σ (inductive_mind ind) = Some pars.
-Proof.
-  rewrite /lookup_constructor_pars_args /lookup_inductive_pars.
-  rewrite /lookup_inductive. destruct lookup_minductive => //.
-  cbn. do 2 destruct nth_error => //. congruence.
-Qed.
-
-Lemma eval_mkApps_Construct {fl : Ee.WcbvFlags} Σ kn c args args' : 
-  All2 (Ee.eval Σ) args args' ->
-  Ee.eval Σ (mkApps (tConstruct kn c) args) (mkApps (tConstruct kn c) args').
-Proof.
-  revert args'. induction args using rev_ind; intros args'; destruct args' using rev_case; intros a.
-  - depelim a. constructor => //.
-  - depelim a. cbn. now apply app_tip_nil in H.
-  - depelim a. now apply app_tip_nil in H.
-  - eapply All2_app_inv in a as []. 2:{ eapply All2_length in a. len in a. cbn in a. lia. } 
-    depelim a0. clear a0. rewrite !mkApps_app /=.
-    constructor; auto.
-    destruct args' using rev_ind; try now rewrite ?mkApps_app; cbn; destruct Ee.with_guarded_fix; eauto.
-    cbn. rewrite Ee.isFixApp_mkApps; eauto.
-    cbn. try now rewrite ?mkApps_app; cbn; destruct Ee.with_guarded_fix; eauto.
-Qed.
-
-Arguments isEtaExp : simpl never.
-
-Lemma isEtaExp_tApp' {Σ} {Γ} {f u} : isEtaExp Σ Γ (tApp f u) -> 
-  let (hd, args) := decompose_app (tApp f u) in
-  match expanded_head_viewc hd with
-  | expanded_head_construct kn c =>
-    args <> [] /\ f = mkApps hd (remove_last args) /\ u = last args u /\ 
-    isEtaExp_app Σ kn c #|args| && forallb (isEtaExp Σ Γ) args
-  | expanded_head_fix mfix idx => 
-    args <> [] /\ f = mkApps hd (remove_last args) /\ u = last args u /\ 
-    isEtaExp_fixapp mfix idx #|args| && forallb (fun d => isEtaExp Σ (rev_map (fun  d => 1 + d.(rarg)) mfix ++ Γ) d.(dbody)) mfix && forallb (isEtaExp Σ Γ) args
-  | expanded_head_rel n => 
-    args <> [] /\ f = mkApps hd (remove_last args) /\ u = last args u /\ 
-    option_default (fun m => m <=? List.length args) (nth_error Γ n) false && forallb (fun x => isEtaExp Σ Γ x) args
-  | expanded_head_other _ discr => 
-    [&& isEtaExp Σ Γ hd, forallb (isEtaExp Σ Γ) args, isEtaExp Σ Γ f & isEtaExp Σ Γ u]
-  end.
-Proof.
-  move/(isEtaExp_tApp Σ Γ f [u]).
-  cbn -[decompose_app]. destruct decompose_app eqn:da.
-  destruct expanded_head_viewc eqn:cv => //.
-  - intros ->.
-    pose proof (decompose_app_inv da).
-    pose proof (decompose_app_notApp _ _ _ da).
-    destruct l using rev_case. cbn. intuition auto. solve_discr. noconf H.
-    rewrite mkApps_app in H. noconf H.
-    rewrite remove_last_app last_last. intuition auto.
-    destruct l; cbn in *; congruence.
-  - intros Hfix.
-    pose proof (decompose_app_inv da).
-    pose proof (decompose_app_notApp _ _ _ da).
-    destruct l using rev_case. cbn. intuition auto. solve_discr. noconf H. noconf H.
-    rewrite mkApps_app in H. noconf H.
-    rewrite remove_last_app last_last. intuition auto.
-    destruct l; cbn in *; congruence.
-  - intros ->.
-    pose proof (decompose_app_inv da).
-    pose proof (decompose_app_notApp _ _ _ da).
-    destruct l using rev_case. cbn. intuition auto. solve_discr. noconf H.
-    rewrite mkApps_app in H. noconf H.
-    rewrite remove_last_app last_last. intuition auto.
-    destruct l; cbn in *; congruence.
-  - pose proof (decompose_app_inv da).
-    pose proof (decompose_app_notApp _ _ _ da).
-    destruct l using rev_case. cbn. intuition auto. destruct t => //.
-    rewrite mkApps_app in H. noconf H.
-    move=> /andP[] etat. rewrite forallb_app => /andP[] etal /=.
-    rewrite andb_true_r => etaa. rewrite etaa andb_true_r.
-    rewrite etat etal. cbn. rewrite andb_true_r.
-    eapply isEtaExp_mkApps_intro; auto; solve_all.
-Qed.
-
-Lemma decompose_app_tApp_split f a hd args :
-  decompose_app (tApp f a) = (hd, args) -> f = mkApps hd (remove_last args) /\ a = last args a.
-Proof.
-  unfold decompose_app. cbn.
-  move/decompose_app_rec_inv' => [n [napp [hskip heq]]].
-  rewrite -(firstn_skipn n args).
-  rewrite -hskip. rewrite last_last; split => //.
-  rewrite heq. f_equal.
-  now rewrite remove_last_app.
-Qed.
-
-Lemma isEtaExp_lookup_ext {Σ} {kn d}: 
-  isEtaExp_env Σ ->
-  lookup_env Σ kn = Some d ->
-  ∑ Σ', extends Σ' Σ × isEtaExp_decl Σ' d.
-Proof.
-  induction Σ; cbn.
-  - move=> _; rewrite /declared_constant /lookup_env /= //.
-  - move=> /andP[] etaa etaΣ.
-    destruct a as [kn' d']; cbn in *.
-    elim: eqb_specT.
-    * intros ?; subst kn'. move=> [=]. intros ->.
-      exists Σ. split => //. now exists [(kn, d)].
-    * intros hkn; move=> Hl. destruct (IHΣ etaΣ Hl) as [Σ' [ext eta]].
-      exists Σ'; split => //.
-      destruct ext as [Σ'' ->].
-      now exists ((kn', d')::Σ'').
-Qed.
-
-Lemma isEtaExp_app_extends Σ Σ' ind k n :
-  extends Σ Σ' ->
-  wf_glob Σ' -> 
-  isEtaExp_app Σ ind k n ->
-  isEtaExp_app Σ' ind k n.
-Proof.
-  rewrite /isEtaExp_app.
-  rewrite /lookup_constructor_pars_args /lookup_inductive /lookup_minductive.
-  move=> ext wf.
-  destruct (lookup_env Σ _) eqn:hl => //.
-  rewrite (extends_lookup wf ext hl) /= //.
-Qed.
-
-Lemma isEtaExp_extends Σ Σ' Γ t : 
-  extends Σ Σ' ->
-  wf_glob Σ' ->
-  isEtaExp Σ Γ t ->
-  isEtaExp Σ' Γ t.
-Proof.
-  intros ext wf.
-  funelim (isEtaExp Σ Γ t); simp_eta => //; rtoProp; intuition eauto; rtoProp; intuition auto.
-  - eapply In_All in H; solve_all.
-  - eapply isEtaExp_app_extends; tea.
-  - eapply In_All in H0. solve_all.
-  - eapply In_All in H; solve_all.
-  - eapply In_All in H; solve_all.
-    rewrite isEtaExp_Constructor //. rtoProp; intuition auto.
-    eapply isEtaExp_app_extends; tea.
-    solve_all.
-  - eapply In_All in H, H0. rewrite isEtaExp_mkApps => //.
-    cbn [expanded_head_viewc]. rtoProp. repeat split; eauto.
-    all: solve_all.
-  - eapply In_All in H. rewrite isEtaExp_mkApps => //.
-    cbn [expanded_head_viewc]. rtoProp. repeat split; eauto.
-    all: solve_all.
-  - eapply In_All in H0. apply isEtaExp_mkApps_intro; eauto. solve_all.
-Qed.
-
-Lemma isEtaExp_extends_decl Σ Σ' t : 
-  extends Σ Σ' ->
-  wf_glob Σ' ->
-  isEtaExp_decl Σ t ->
-  isEtaExp_decl Σ' t.
-Proof.
-  intros ext wf; destruct t; cbn => //.
-  rewrite /isEtaExp_constant_decl; destruct (cst_body c) => /= //.
-  now eapply isEtaExp_extends.
-Qed.
-
-Lemma isEtaExp_lookup {Σ kn d}: 
-  isEtaExp_env Σ -> wf_glob Σ ->
-  lookup_env Σ kn = Some d ->
-  isEtaExp_decl Σ d.
-Proof.
-  move=> etaΣ wfΣ.
-  move/(isEtaExp_lookup_ext etaΣ) => [Σ' []] ext hd.
-  now eapply isEtaExp_extends_decl.
-Qed.
-
-Arguments lookup_inductive_pars_constructor_pars_args {Σ ind n pars args}.
-
-Lemma Forall_last {A} (P : A -> Prop) a l : l <> [] -> Forall P l -> P (last l a).
-Proof.
-  intros. induction H0.
-  - congruence.
-  - destruct l.
-    + cbn. eauto.
-    + cbn. eapply IHForall. congruence.
-Qed.
-
-Lemma All_remove_last {A} (P : A -> Type) l : All P l -> All P (remove_last l).
-Proof.
-  intros. now eapply All_firstn.
-Qed.
-
-Lemma eval_etaexp {fl : Ee.WcbvFlags} {Σ a a'} : 
-  isEtaExp_env Σ ->
-  wf_glob Σ ->
-  Ee.eval Σ a a' -> isEtaExp Σ [] a -> isEtaExp Σ [] a'.
-Proof.
-  intros etaΣ wfΣ.
-  induction 1 as [ | ? ? ? ? ? ? ? ? IHs | | | | ? ? ? ? ? ? ? ? ? ? ? IHs | ? ? ? ? ? ? ? ? ? ? ? IHs | ? ? ? ? ? ? ? ? ? ? IHs | | | | | | |   ] using eval_mkApps_rect.
-  all:try simp isEtaExp; rewrite -!isEtaExp_equation_1 => //.
-  6:{  
-    move/isEtaExp_tApp'.
-    destruct decompose_app eqn:da.
-    destruct expanded_head_viewc eqn:vc.
-    * move => [hl [hf [ha /andP[] ise etal]]].
-      pose proof (H' := H).
-      rewrite hf in H'. eapply eval_construct in H' as [? []]. exfalso. solve_discr.
-    * move => [hl [hf [ha /andP[] /andP[] etal etab]]] isel.
-      pose proof (mkApps_app (EAst.tFix mfix idx) argsv [av]).
-      cbn in H3. rewrite <- H3. clear H3.
-      subst.
-      specialize eval_mkApps_tFix_inv_size with (Heval := H); intros [(args' & ? & Heq) | (? & ? & ? & ? & ?)]; eauto.
-      -- eapply (f_equal decompose_app) in Heq. rewrite !decompose_app_mkApps in Heq => //. invs Heq.
-         rewrite isEtaExp_mkApps => //.
-         cbn [expanded_head_viewc]. rtoProp. repeat split.
-         ++ unfold isEtaExp_fixapp in *. destruct nth_error eqn:Hn; try easy. len.
-            eapply Nat.ltb_lt in etal.
-            eapply Nat.ltb_lt. eapply Forall2_length in H3.
-            rewrite remove_last_length' in H3 |-*. eauto. lia.
-         ++ solve_all.
-         ++ sq. solve_all. eapply All_app_inv. 2:{ repeat econstructor. eapply IHeval2. rewrite ha. eapply Forall_last; eauto. }
-            eapply All_remove_last in isel.
-            solve_all. destruct b.
-            unshelve eapply IHs. 2: eauto. lia. eauto.
-       -- rewrite !isEtaExp_mkApps in IHeval1 |- * => //.
-          cbn [expanded_head_viewc] in *. forward IHeval1; rtoProp.
-          ++ repeat split; solve_all. 2:{ unfold remove_last. now eapply All_firstn. }
-             unfold isEtaExp_fixapp, cunfold_fix in *. destruct nth_error; invs H1. clear IHeval1.
-             destruct nth_error; invs H4. eapply Nat.ltb_lt in etal. eapply Nat.ltb_lt. len.
-             destruct l; try congruence.
-          ++ repeat split; solve_all. 2:{ eapply All_app_inv; eauto. repeat econstructor; eauto. eapply IHeval2. rewrite ha. eapply Forall_last; eauto. }
-             unfold isEtaExp_fixapp, cunfold_fix in *. destruct nth_error; invs H1.
-             destruct nth_error; invs H4. eapply Nat.ltb_lt in H6, etal. eapply Nat.ltb_lt. len.
-             destruct l; try congruence. cbn. rewrite remove_last_length' in H5; try congruence. cbn in *. lia.
-      * intros (? & ? & ? & ?). rtoProp. solve_all.
-        rewrite nth_error_nil in H6. easy.
-      * move/and4P => [] etat etal etaf etaa.
-        pose proof (mkApps_app (tFix mfix idx) argsv [av]). cbn in H3. rewrite <- H3. clear H3.
-        specialize (IHeval1 etaf). 
-        rewrite !isEtaExp_mkApps in IHeval1 |- * => //.
-        cbn [expanded_head_viewc] in *. rtoProp. repeat split; solve_all.
-        -- unfold isEtaExp_fixapp, cunfold_fix in *. destruct nth_error; invs H1.
-           len. eapply Nat.ltb_lt. eapply Nat.ltb_lt in H3. lia.
-        -- eapply All_app_inv; solve_all.
-  }
-  5:{
-    move/isEtaExp_tApp'.
-    destruct decompose_app eqn:da.
-    destruct expanded_head_viewc eqn:vc.
-    * move => [hl [hf [ha /andP[] ise etal]]]. clear IHs.
-      rewrite hf in H. eapply eval_construct in H as [? []]. exfalso. solve_discr.
-    * move => [hl [hf [ha /andP[] /andP[] etal etab]]] isel.
-      subst.
-      eapply IHeval3.
-      
-      pose proof (mkApps_app fn argsv [av]).
-      cbn in H3. rewrite <- H3. clear H3.
-
-      assert (isEtaExp Σ [] a). { rewrite ha. eapply Forall_last; eauto. solve_all. }
-
-      specialize eval_mkApps_tFix_inv_size with (Heval := H); intros [(args' & ? & Heq) | (? & ? & ? & ? & ?)]; eauto.
-      -- solve_all. eapply (f_equal decompose_app) in Heq. rewrite !decompose_app_mkApps in Heq => //. invs Heq. sq.
-         eapply isEtaExp_mkApps_intro. 
-         eapply isEtaExp_cunfold_fix. 2: eauto. solve_all.
-         now rewrite app_nil_r in H6.
-         eapply All_app_inv. 2: repeat econstructor; eauto.
-         eapply All_remove_last in isel.
-         solve_all. destruct b.
-         unshelve eapply IHs. 2: eauto. lia. eauto.
-       -- forward IHeval1.
-          rewrite isEtaExp_mkApps => //.
-          cbn [expanded_head_viewc]. rtoProp. repeat split; solve_all.
-          2: eapply All_firstn; eauto.
-          unfold isEtaExp_fixapp, cunfold_fix in *.
-          destruct nth_error; try easy. invs H1.
-          destruct nth_error; try easy. invs H5. eapply Nat.ltb_lt. lia.
-          rewrite isEtaExp_mkApps in IHeval1 => //.
-          cbn [expanded_head_viewc] in IHeval1. rtoProp.
-          eapply isEtaExp_mkApps_intro. 
-          eapply isEtaExp_cunfold_fix. 2: eauto. solve_all.
-          now rewrite app_nil_r in H10.
-          eapply All_app_inv. 2: repeat econstructor; eauto.
-          solve_all.
-        * intros (? & ? & ? & ?). rtoProp. solve_all.
-          rewrite nth_error_nil in H6. easy.
-        * move/and4P => [] etat etal etaf etaa. eapply IHeval3.
-          pose proof (mkApps_app fn argsv [av]). cbn in H3. rewrite <- H3. clear H3.
-          specialize (IHeval1 etaf). 
-          rewrite !isEtaExp_mkApps in IHeval1 => //.
-          cbn [expanded_head_viewc] in *. rtoProp.
-          eapply isEtaExp_mkApps_intro. 
-          eapply isEtaExp_cunfold_fix. 2: eauto. solve_all.
-          now rewrite app_nil_r in H6.
-          eapply All_app_inv. 2: repeat econstructor; eauto.
-          solve_all.
-  }
-  10:{ move/isEtaExp_tApp'.
-  destruct decompose_app eqn:da.
-  destruct expanded_head_viewc.
-  * move=> [] hl [] hf [] ha /andP[] hl' etal.
-    move: H H0. rewrite hf => H H0.
-    destruct (eval_construct_size H) as [args' []]. subst f'.
-    rewrite -[EAst.tApp _ _](mkApps_app _ _ [a']).
-    rewrite isEtaExp_Constructor.
-    apply/andP; split => //.
-    + len. eapply All2_length in a0. rewrite -a0.
-      rewrite (remove_last_last l a) // in hl'.
-      rewrite app_length in hl'.
-      now cbn in hl'.
-    + solve_all.
-      rewrite (remove_last_last l a) // in etal.
-      eapply All_app in etal as [etal etaa].
-      depelim etaa. clear etaa. rewrite -ha in i.
-      eapply All_app_inv; try constructor; eauto.
-      clear -H0 a0 etal. solve_all.
-      destruct b as [ev Hev]. eapply (H0 _ _ ev) => //. lia.
-  * move => [hl [hf [ha /andP[] /andP[] etal etab]]] isel.
-    subst.
-  
-    assert (isEtaExp Σ [] a). { rewrite ha. eapply Forall_last; solve_all. }
-    destruct with_guarded_fix eqn:guarded.
-    {
-    
-    specialize eval_mkApps_tFix_inv_size with (Heval := H); intros [(args' & ? & Heq) | (? & ? & ? & ? & ?)]; eauto.
-    -- subst. rewrite isFixApp_mkApps in H1 => //. destruct EAst.isLambda; easy.
-    -- eapply (isEtaExp_mkApps_intro _ _ f' [a']); eauto.
-       eapply IHeval1. rewrite isEtaExp_mkApps => //.
-      cbn [expanded_head_viewc]. rtoProp.
-      repeat split; solve_all.
-      2: eapply All_firstn; eauto.
-      unfold isEtaExp_fixapp,  cunfold_fix in *.
-      destruct nth_error; try easy.
-      invs H5. eapply Nat.ltb_lt. lia.
-
-    }
-    {
-      specialize eval_mkApps_tFix_inv_size_unguarded with (Heval := H); intros Hinv; destruct Hinv as [[Heq ->] | (a_ & args' & argsv & Heq & Hall & n & fn & Hunf & Hev & Hsz)]; eauto.
-      -- cbn in *. easy.
-      -- eapply (isEtaExp_mkApps_intro _ _ f' [a']); eauto.
-         unshelve eapply H0. 2: eauto. lia.
-         eapply (isEtaExp_mkApps_intro).
-         eapply (isEtaExp_mkApps_intro _ _ fn [a_]); eauto. 2: econstructor; [ | econstructor].
-         ++ eapply isEtaExp_cunfold_fix. 2: eauto. solve_all. now rewrite app_nil_r in H5.
-         ++ solve_all. eapply All_firstn in isel. unfold remove_last in Heq. eapply All_Forall in isel.
-            setoid_rewrite Heq in isel. invs isel. eauto.
-         ++ eapply forallb_Forall in isel. eapply Forall_firstn in isel. unfold remove_last in Heq.
-            setoid_rewrite Heq in isel. eapply Forall_All in isel. invs isel. solve_all. subst; eauto.
-            destruct H6. unshelve eapply H0. 2: eauto. lia. eauto.
-       }
-  * intros (? & ? & ? & ?). rtoProp. solve_all.
-      rewrite nth_error_nil in H6. easy.
-  * move/and4P => [] etat etal etaf etaa. 
-  eapply (isEtaExp_mkApps_intro _ _ f' [a']); eauto.
-  }
-  1:{ move/isEtaExp_tApp'.
-      destruct decompose_app eqn:da.
-      destruct expanded_head_viewc.
-      * clear IHs. move=> [] hl [] hf [] ha /andP[] hl' etal.
-        move: H H0. rewrite hf => H H0.
-        eapply eval_construct in H as [? []];solve_discr.
-      * solve_all. rtoProp. solve_all. subst.
-
-      destruct with_guarded_fix eqn:guarded.
-
-      {
-        specialize eval_mkApps_tFix_inv_size with (Heval := H); intros [(args' & ? & Heq) | (? & ? & ? & ? & ?)]; eauto. 
-        -- solve_discr.
-        -- eapply IHeval3. eapply etaExp_csubst. eapply IHeval2.
-           rewrite H3. eapply Forall_last; solve_all.
-           forward IHeval1.
-           rewrite isEtaExp_mkApps => //.
-           cbn [expanded_head_viewc]. rtoProp; solve_all; solve_all.
-           2: eapply All_firstn; solve_all.
-           unfold isEtaExp_fixapp, cunfold_fix in *.
-           destruct nth_error; try easy. invs H8. eapply Nat.ltb_lt. lia.
-           simp_eta in IHeval1. eauto.
-      }
-      {
-        specialize eval_mkApps_tFix_inv_size_unguarded with (Heval := H); intros Hinv; destruct Hinv as [[Heq Heq'] | (a_ & args' & argsv & Heq & Hall & n & fn & Hunf & Hev & Hsz)]; eauto; try congruence.
-        eapply IHeval3. eapply etaExp_csubst.
-        
-        eapply IHeval2. rewrite H3. eapply Forall_last. eauto. solve_all. 
-        assert (isEtaExp Σ [] (mkApps (tApp fn a_) argsv) -> isEtaExp Σ []  (EAst.tLambda na b)) as IH. {
-         unshelve eapply IHs; eauto.
-        }
-        simp_eta in IH. eapply IH.
-        eapply (isEtaExp_mkApps_intro).
-        eapply (isEtaExp_mkApps_intro _ _ fn [a_]); eauto. 2: econstructor; [ | econstructor].
-        ++ eapply isEtaExp_cunfold_fix. 2: eauto. solve_all. now rewrite app_nil_r in H4.
-        ++ solve_all. eapply All_firstn in H6 as isel. unfold remove_last in Heq. eapply All_Forall in isel.
-           setoid_rewrite Heq in isel. invs isel. eauto.
-        ++ eapply All_Forall in H6 as isel. eapply Forall_firstn in isel. unfold remove_last in Heq.
-           setoid_rewrite Heq in isel. eapply Forall_All in isel. invs isel. solve_all. subst; eauto.
-           destruct H4. unshelve eapply IHs. 2: eauto. lia. eauto.        
-      }
-     
-       * solve_all. rtoProp. solve_all. rewrite nth_error_nil in H5; easy.
-  * move/and4P => [] etat etal etaf etaa. simp_eta in IHeval1. eapply IHeval3, etaExp_csubst; eauto.  
-  }
-
-  - rtoProp. solve_all. eapply IHeval2, etaExp_csubst; eauto. 
-
-  - rtoProp; intuition eauto.
-    eapply IHeval2. rewrite /iota_red.
-    eapply isEtaExp_substl with (Γ := repeat 0 #|br.1|); eauto.
-    { len. lia. }
-    rewrite isEtaExp_Constructor // in H4. solve_all.
-    eapply All_skipn. move/andP: H4 => []. repeat solve_all.
-    eapply forallb_nth_error in H6; tea.
-    now erewrite H1 in H6.
-  - rtoProp; intuition auto.
-    eapply IHeval2. eapply isEtaExp_substl. shelve.
-    now apply forallb_repeat.
-    rewrite H2 in H6. simpl in H6.
-    now move/andP: H6.
-    Unshelve. now len.
-  - move/isEtaExp_tApp'.
-    destruct decompose_app eqn:da.
-    destruct expanded_head_viewc.
-    * clear IHs. move=> [] hl [] hf [] ha /andP[] hl' etal.
-      move: H H0. rewrite hf => H H0.
-      eapply eval_construct in H as [? []];solve_discr.
-    * solve_all. rtoProp. solve_all. subst.
-      specialize eval_mkApps_tFix_inv_size_unguarded with (Heval := H); intros Hinv; destruct Hinv as [[Heq Heq'] | (a_ & args' & argsv & Heq & Hall & n & fn_ & Hunf & Hev & Hsz)]; eauto; try congruence.
-
-      -- invs Heq'. eapply IHeval2. 
-         eapply (isEtaExp_mkApps_intro _ _ fn [a]); eauto. 2: econstructor; [ | econstructor].
-         ++ eapply isEtaExp_cunfold_fix. 2: eauto. solve_all. now rewrite app_nil_r in H4.
-         ++ rewrite H3. eapply Forall_last. 2: solve_all. eauto.
-      -- assert (isEtaExp Σ [] (mkApps (tApp fn_ a_) argsv) -> isEtaExp Σ [] (EAst.tFix mfix idx)). { eapply IHs; eauto. }
-         exfalso.
-         forward H4.
-         eapply isEtaExp_mkApps_intro. 
-         eapply (isEtaExp_mkApps_intro _ _ fn_ [a_]); eauto. 2: econstructor; [ | econstructor].
-         ** eapply isEtaExp_cunfold_fix. 2: eauto. solve_all. now rewrite app_nil_r in H7.
-         ** solve_all. eapply All_firstn in H6 as isel. unfold remove_last in Heq. eapply All_Forall in isel.
-            setoid_rewrite Heq in isel. invs isel. eauto.
-         ** eapply All_firstn in H6 as isel. unfold remove_last in Heq. eapply All_Forall in isel.
-            setoid_rewrite Heq in isel. eapply Forall_All in isel. invs isel. solve_all; subst; eauto.
-            destruct H8.
-            unshelve eapply IHs. 2: eauto. lia. eauto.
-         ** simp_eta in H3. easy.
-    * solve_all. rtoProp. solve_all. rewrite nth_error_nil in H5. easy.
-    * move/and4P => [] etat etal etaf etaa.
-      forward IHeval1. eauto.
-      simp_eta in IHeval1. easy.
-  - move=> /andP[] hdiscr hbrs. specialize (IHeval1 hdiscr).
-    move: IHeval1. rewrite isEtaExp_mkApps // /= => /andP[] hcof hargs.
-    eapply IHeval2. simp_eta. rtoProp; intuition auto.
-    apply isEtaExp_mkApps_intro; solve_all.
-    eapply (isEtaExp_cunfold_cofix _ mfix idx); tea.
-    simp_eta in hcof. solve_all. now rewrite app_nil_r in H2.
-  - move=> hdiscr. specialize (IHeval1 hdiscr).
-    move: IHeval1. rewrite isEtaExp_mkApps // /= => /andP[] hcof hargs.
-    eapply IHeval2. simp_eta.
-    apply isEtaExp_mkApps_intro; solve_all.
-    eapply (isEtaExp_cunfold_cofix _ mfix idx); tea.
-    simp_eta in hcof. solve_all. now rewrite app_nil_r in H2.
-  - move=> _. eapply IHeval. eapply isEtaExp_lookup in H; tea.
-    now move: H; rewrite /isEtaExp_decl /= /isEtaExp_constant_decl H0 /=.
-  - intros hd.
-    eapply IHeval2. specialize (IHeval1 hd).
-    move: IHeval1.
-    rewrite nth_nth_error in H1 *.
-    destruct nth_error eqn:hnth.
-    rewrite isEtaExp_Constructor.
-    destruct args => //. now rewrite nth_error_nil in hnth.
-    move=> /andP[] _ hargs.
-    eapply nth_error_forallb in hnth; tea.
-    depelim H0. now cbn in H1. Unshelve.
-Qed.
-
-(* Lemma isEtaExp_eval Σ {wfl : WcbvFlags} t v  :
-eval Σ t v -> isEtaExp Σ [] t -> isEtaExp Σ [] v.
-Admitted.
-
-Local Arguments eval : clear implicits.
-
-Lemma eval_opt_to_target Σ t v  :
-@eval opt_wcbv_flags Σ t v -> isEtaExp Σ [] t -> @eval target_wcbv_flags Σ t v.
-Proof.
-intros H. depind H; intros Hexp; eauto.
-- todo "box".
-- todo "lambda".
-- simp_eta in Hexp. rtoProp. econstructor. eauto. eapply IHeval2. todo "isEtaExp csubst".
-- todo "case".
-- todo "case".
-- destruct argsv.
-  + cbn -[isEtaExp] in *. todo "impossible due to expansion".
-  + eapply eval_trans. eapply eval_app_cong.
-    * eapply IHeval1. todo "exp".
-    * cbn. destruct argsv using rev_ind; cbn; try eauto. now rewrite mkApps_app. 
-    * eapply IHeval2. todo "exp". 
-    * replace (tApp (mkApps fn (t :: argsv)) av) with (mkApps (tApp fn t) (argsv ++ [av])) in IHeval3 by now rewrite mkApps_app.
-      replace (tApp (mkApps (tFix mfix idx) (t :: argsv)) av) with (mkApps (tApp (tFix mfix idx) t) (argsv ++ [av])) by now rewrite mkApps_app.
-      forward IHeval3. todo "exp".
-      revert IHeval3. generalize (argsv ++ [av])%list. clear - e. intros l.
-      revert res.
-      induction l using rev_ind.
-      -- cbn in *. intros. eapply eval_fix'; eauto.
-      -- rewrite !mkApps_app; cbn. intros res H.
-         eapply eval_trans.
-         eapply eval_mkApps_inv with (args := [x]) in H as (? & ? & ?).
-         eapply eval_app_cong_tApp. eapply IHl; eauto.
-         cbn in *. eauto.
-         eapply value_final, eval_to_value; eauto.
-- todo "impossible due to expansion".
-- cbn in unguarded. congruence.
-- todo "case".
-- todo "proj".
-- todo "const".
-- todo "proj".
-- todo "proj".
-- eapply eval_app_cong => //.
-  + eapply IHeval1. todo "exp".
-  + destruct f'; cbn in *; eauto.
-  + eapply IHeval2. todo "exp".
-Qed. *)
