erasure/theories/EEnvMap.v
@@ -1,0 +1,44 @@
+From Coq Require Import ssreflect ssrbool.
+From MetaCoq.Template Require Import utils Kernames EnvMap.
+From MetaCoq.Erasure Require Import EAst EGlobalEnv EAstUtils EGlobalEnv EAstUtils.
+Import MCMonadNotation.
+
+Module GlobalContextMap.
+  Record t := 
+  { global_decls :> global_declarations; 
+    map : EnvMap.t global_decl;
+    repr : EnvMap.repr global_decls map;
+    wf : EnvMap.fresh_globals global_decls }.
+  
+  Definition lookup_minductive Σ kn : option mutual_inductive_body :=
+    decl <- EnvMap.lookup kn Σ.(map);; 
+    match decl with
+    | ConstantDecl _ => None
+    | InductiveDecl mdecl => ret mdecl
+    end.
+
+  Definition lookup_inductive Σ kn : option (mutual_inductive_body * one_inductive_body) :=
+    mdecl <- lookup_minductive Σ (inductive_mind kn) ;;
+    idecl <- nth_error mdecl.(ind_bodies) (inductive_ind kn) ;;
+    ret (mdecl, idecl).
+  
+  Definition lookup_inductive_pars Σ kn : option nat := 
+    mdecl <- lookup_minductive Σ kn ;;
+    ret mdecl.(ind_npars).
+
+  Lemma lookup_inductive_pars_spec Σ kn : lookup_inductive_pars Σ kn = EGlobalEnv.lookup_inductive_pars Σ kn.
+  Proof.
+    rewrite /lookup_inductive_pars /EGlobalEnv.lookup_inductive_pars.
+    rewrite /lookup_inductive /EGlobalEnv.lookup_inductive.
+    rewrite /lookup_minductive /EGlobalEnv.lookup_minductive.
+    rewrite (EnvMap.lookup_spec Σ.(global_decls)).
+    eapply wf. eapply repr. reflexivity.
+  Qed.
+
+  Program Definition make (g : global_declarations) (Hg : EnvMap.fresh_globals g): t :=
+    {| global_decls := g;
+       map := EnvMap.of_global_env g |}.
+
+End GlobalContextMap.
+
+Coercion GlobalContextMap.global_decls : GlobalContextMap.t >-> global_declarations.
