erasure/theories/EWcbvEvalInd.v
@@ -1,7 +1,7 @@
 (* Distributed under the terms of the MIT license. *)
 From Coq Require Import Utf8 Program ssreflect ssrbool.
 From MetaCoq.Template Require Import config utils Kernames BasicAst EnvMap.
-From MetaCoq.Erasure Require Import EAst EAstUtils EInduction EWcbvEval ETyping ECSubst EInduction.
+From MetaCoq.Erasure Require Import EAst EAstUtils EInduction EWcbvEval EGlobalEnv ECSubst EInduction.
 
 Set Asymmetric Patterns.
 From Equations Require Import Equations.
