erasure/theories/ErasureCorrectness.v
@@ -1,7 +1,7 @@
 (* Distributed under the terms of the MIT license. *)
 From Coq Require Import Program.
 From MetaCoq.Template Require Import config utils.
-From MetaCoq.Erasure Require Import ELiftSubst ETyping EWcbvEval Extract Prelim
+From MetaCoq.Erasure Require Import ELiftSubst EGlobalEnv EWcbvEval Extract Prelim
      ESubstitution EInversion EArities EDeps.
 From MetaCoq.PCUIC Require Import PCUICTyping PCUICGlobalEnv PCUICAst
   PCUICAstUtils PCUICConversion PCUICSigmaCalculus
@@ -759,7 +759,7 @@ Qed.
 
 Lemma isPropositional_propositional Σ Σ' ind mdecl idecl mdecl' idecl' : 
   PCUICAst.declared_inductive Σ ind mdecl idecl ->
-  ETyping.declared_inductive Σ' ind mdecl' idecl' ->
+  EGlobalEnv.declared_inductive Σ' ind mdecl' idecl' ->
   erases_mutual_inductive_body mdecl mdecl' ->
   erases_one_inductive_body idecl idecl' ->
   forall b, isPropositional Σ ind b -> inductive_isprop_and_pars Σ' ind = Some (b, mdecl.(ind_npars)).
@@ -1399,7 +1399,7 @@ Proof.
       invs H2.
       -- exists x2. split; eauto.
          constructor. econstructor. eauto. 2:eauto.
-         3:{ unfold ETyping.iota_red.
+         3:{ unfold EGlobalEnv.iota_red.
           rewrite ECSubst.substl_subst //.
           eapply Forall_rev, Forall_skipn.
           assert (Forall (closedn 0) args).
@@ -1637,7 +1637,7 @@ Proof.
 
         enough (Σ;;; [] ,,, subst_context (fix_subst mfix) 0 []
                 |- subst (fix_subst mfix) 0 dbody
-                ⇝ℇ ELiftSubst.subst (ETyping.fix_subst mfix') 0 (Extract.E.dbody x4)).
+                ⇝ℇ ELiftSubst.subst (EGlobalEnv.fix_subst mfix') 0 (Extract.E.dbody x4)).
         destruct p. destruct p.
 
         clear e3. rename H into e3.
@@ -1695,7 +1695,7 @@ Proof.
            ++ eauto.
            ++ eauto.
            ++ rewrite <- Ee.closed_unfold_fix_cunfold_eq.
-              { unfold ETyping.unfold_fix. rewrite e -e4.
+              { unfold EGlobalEnv.unfold_fix. rewrite e -e4.
                 now rewrite (Forall2_length H4). }
               eapply eval_closed in e3; eauto.
               clear -e3 Hmfix'.
@@ -1724,7 +1724,7 @@ Proof.
            ++ eapply nth_error_all in a1; eauto. cbn in a1.
               eapply a1.
            ++ eapply All2_from_nth_error.
-              erewrite fix_subst_length, ETyping.fix_subst_length, All2_length; eauto.
+              erewrite fix_subst_length, EGlobalEnv.fix_subst_length, All2_length; eauto.
               intros.
               rewrite fix_subst_nth in H3. now rewrite fix_subst_length in H2.
               rewrite efix_subst_nth in H5. rewrite fix_subst_length in H2.
@@ -1878,7 +1878,7 @@ Proof.
         { eapply All2_nth_error_Some in X0 as X'; tea.
           destruct X' as [t' [nth' [bn [rar eb]]]].
           specialize (IHeval2 (E.tCase (ip, ci_npar ip) 
-            (E.mkApps (ELiftSubst.subst0 (ETyping.cofix_subst mfix') (E.dbody t')) L') brs')).
+            (E.mkApps (ELiftSubst.subst0 (EGlobalEnv.cofix_subst mfix') (E.dbody t')) L') brs')).
           forward IHeval2.
           econstructor; eauto.
           eapply erases_mkApps.
@@ -1890,7 +1890,7 @@ Proof.
           { rewrite app_context_nil_l. eapply subslet_cofix_subst; eauto.
             econstructor; eauto. }
           {eapply All2_from_nth_error.
-            erewrite cofix_subst_length, ETyping.cofix_subst_length, All2_length; eauto.
+            erewrite cofix_subst_length, EGlobalEnv.cofix_subst_length, All2_length; eauto.
             intros.
             rewrite cofix_subst_nth in H3. now rewrite cofix_subst_length in H2.
             rewrite ecofix_subst_nth in H8. rewrite cofix_subst_length in H2.
@@ -1997,7 +1997,7 @@ Proof.
         { eapply All2_nth_error_Some in X as X'; tea.
           destruct X' as [t' [nth' [bn [rar eb]]]].
           specialize (IHeval2 (E.tProj p
-            (E.mkApps (ELiftSubst.subst0 (ETyping.cofix_subst mfix') (E.dbody t')) L'))).
+            (E.mkApps (ELiftSubst.subst0 (EGlobalEnv.cofix_subst mfix') (E.dbody t')) L'))).
           forward IHeval2.
           econstructor; eauto.
           eapply erases_mkApps.
@@ -2009,7 +2009,7 @@ Proof.
           { rewrite app_context_nil_l. eapply subslet_cofix_subst; eauto.
             econstructor; eauto. }
           {eapply All2_from_nth_error.
-            erewrite cofix_subst_length, ETyping.cofix_subst_length, All2_length; eauto.
+            erewrite cofix_subst_length, EGlobalEnv.cofix_subst_length, All2_length; eauto.
             intros.
             rewrite cofix_subst_nth in H4. now rewrite cofix_subst_length in H1.
             rewrite ecofix_subst_nth in H7. rewrite cofix_subst_length in H1.
@@ -2147,7 +2147,7 @@ Proof.
     cbn. apply IHer, wf.
 Qed.
 
-Lemma erases_global_decls_fresh univs {Σ : global_declarations} kn Σ' : fresh_global kn Σ -> erases_global_decls univs Σ Σ' -> ETyping.fresh_global kn Σ'.
+Lemma erases_global_decls_fresh univs {Σ : global_declarations} kn Σ' : fresh_global kn Σ -> erases_global_decls univs Σ Σ' -> EGlobalEnv.fresh_global kn Σ'.
 Proof.
   induction 2; constructor; eauto; now depelim H.
 Qed.
