erasure/theories/Extract.v
@@ -3,7 +3,7 @@ From Coq Require Import Program.
 From MetaCoq.Template Require Import config utils.
 From MetaCoq.PCUIC Require Import PCUICAst PCUICAstUtils PCUICTyping
      PCUICElimination PCUICWcbvEval.
-From MetaCoq.Erasure Require EAst ETyping.
+From MetaCoq.Erasure Require EAst EGlobalEnv.
 
 Module E := EAst.
 
@@ -271,19 +271,19 @@ Inductive erases_deps (Σ : global_env) (Σ' : E.global_declarations) : E.term -
     erases_deps Σ Σ' (E.tApp hd arg)
 | erases_deps_tConst kn cb cb' :
     declared_constant Σ kn cb ->
-    ETyping.declared_constant Σ' kn cb' ->
+    EGlobalEnv.declared_constant Σ' kn cb' ->
     erases_constant_body (Σ, cst_universes cb) cb cb' ->
     (forall body, E.cst_body cb' = Some body -> erases_deps Σ Σ' body) ->
     erases_deps Σ Σ' (E.tConst kn)
 | erases_deps_tConstruct ind c mdecl idecl cdecl mdecl' idecl' cdecl' :
     PCUICAst.declared_constructor Σ (ind, c) mdecl idecl cdecl ->
-    ETyping.declared_constructor Σ' (ind, c) mdecl' idecl' cdecl' ->
+    EGlobalEnv.declared_constructor Σ' (ind, c) mdecl' idecl' cdecl' ->
     erases_mutual_inductive_body mdecl mdecl' ->
     erases_one_inductive_body idecl idecl' ->
     erases_deps Σ Σ' (E.tConstruct ind c)
 | erases_deps_tCase p mdecl idecl mdecl' idecl' discr brs :
     declared_inductive Σ (fst p) mdecl idecl ->
-    ETyping.declared_inductive Σ' (fst p) mdecl' idecl' ->
+    EGlobalEnv.declared_inductive Σ' (fst p) mdecl' idecl' ->
     erases_mutual_inductive_body mdecl mdecl' ->
     erases_one_inductive_body idecl idecl' ->
     erases_deps Σ Σ' discr ->
@@ -291,7 +291,7 @@ Inductive erases_deps (Σ : global_env) (Σ' : E.global_declarations) : E.term -
     erases_deps Σ Σ' (E.tCase p discr brs)
 | erases_deps_tProj p mdecl idecl mdecl' idecl' t :
     declared_inductive Σ p.1.1 mdecl idecl ->
-    ETyping.declared_inductive Σ' p.1.1 mdecl' idecl' ->
+    EGlobalEnv.declared_inductive Σ' p.1.1 mdecl' idecl' ->
     erases_mutual_inductive_body mdecl mdecl' ->
     erases_one_inductive_body idecl idecl' ->
     erases_deps Σ Σ' t ->
